<?xml version="1.0"?>
<rdf:RDF xmlns="http://www.semanticweb.org/djlee/ontologies/2023/8/untitled-ontology-71#"
     xml:base="http://www.semanticweb.org/djlee/ontologies/2023/8/untitled-ontology-71"
     xmlns:dqa="http://local.tamu.edu/djlee/ns/dqa#"
     xmlns:owl="http://www.w3.org/2002/07/owl#"
     xmlns:rdf="http://www.w3.org/1999/02/22-rdf-syntax-ns#"
     xmlns:xml="http://www.w3.org/XML/1998/namespace"
     xmlns:xsd="http://www.w3.org/2001/XMLSchema#"
     xmlns:rdfs="http://www.w3.org/2000/01/rdf-schema#"
     xmlns:skos="http://www.w3.org/2004/02/skos/core#">
    <owl:Ontology rdf:about="http://www.semanticweb.org/djlee/ontologies/2023/8/untitled-ontology-71"/>
    


    <!-- 
    ///////////////////////////////////////////////////////////////////////////////////////
    //
    // Annotation properties
    //
    ///////////////////////////////////////////////////////////////////////////////////////
     -->

    


    <!-- http://www.w3.org/2004/02/skos/core#definition -->

    <owl:AnnotationProperty rdf:about="http://www.w3.org/2004/02/skos/core#definition"/>
    


    <!-- 
    ///////////////////////////////////////////////////////////////////////////////////////
    //
    // Object Properties
    //
    ///////////////////////////////////////////////////////////////////////////////////////
     -->

    


    <!-- http://local.tamu.edu/djlee/ns/dqa#collects -->

    <owl:ObjectProperty rdf:about="http://local.tamu.edu/djlee/ns/dqa#collects">
        <rdfs:domain rdf:resource="https://www.w3.org/TR/prov-o/#Agent"/>
        <rdfs:range rdf:resource="http://local.tamu.edu/djlee/ns/dqa#InformationProduct"/>
        <skos:definition>Indicates A is collected by B (Source: DataCite)</skos:definition>
    </owl:ObjectProperty>
    


    <!-- http://local.tamu.edu/djlee/ns/dqa#contributes -->

    <owl:ObjectProperty rdf:about="http://local.tamu.edu/djlee/ns/dqa#contributes">
        <rdfs:domain rdf:resource="https://www.w3.org/TR/prov-o/#Agent"/>
        <rdfs:range rdf:resource="http://local.tamu.edu/djlee/ns/dqa#InformationProduct"/>
        <skos:definition>Indicate A is contributor of B
(source: PROV Ontology, DataCite)</skos:definition>
    </owl:ObjectProperty>
    


    <!-- http://local.tamu.edu/djlee/ns/dqa#creates -->

    <owl:ObjectProperty rdf:about="http://local.tamu.edu/djlee/ns/dqa#creates">
        <rdfs:domain rdf:resource="https://www.w3.org/TR/prov-o/#Agent"/>
        <rdfs:range rdf:resource="http://local.tamu.edu/djlee/ns/dqa#InformationProduct"/>
        <skos:definition>Indicate A is creator of B
(source: Schema.org, DDI)</skos:definition>
    </owl:ObjectProperty>
    


    <!-- http://local.tamu.edu/djlee/ns/dqa#hasQualityActiveModel -->

    <owl:ObjectProperty rdf:about="http://local.tamu.edu/djlee/ns/dqa#hasQualityActiveModel">
        <rdfs:domain rdf:resource="http://local.tamu.edu/djlee/ns/dqa#InformationProduct"/>
        <rdfs:range rdf:resource="http://local.tamu.edu/djlee/ns/dqa#Quality_Model_Active"/>
        <rdfs:comment>Indicates that a Quality Model is applicable to a specific InformationProduct</rdfs:comment>
    </owl:ObjectProperty>
    


    <!-- http://local.tamu.edu/djlee/ns/dqa#hasQualityProblem -->

    <owl:ObjectProperty rdf:about="http://local.tamu.edu/djlee/ns/dqa#hasQualityProblem">
        <rdfs:domain rdf:resource="http://local.tamu.edu/djlee/ns/dqa#InformationProduct"/>
        <rdfs:range rdf:resource="http://local.tamu.edu/djlee/ns/dqa#Quality_Problem"/>
        <rdfs:comment>Connects inforamtion Product to its Quality Problems.</rdfs:comment>
    </owl:ObjectProperty>
    


    <!-- http://local.tamu.edu/djlee/ns/dqa#hasQualityRequiredModel -->

    <owl:ObjectProperty rdf:about="http://local.tamu.edu/djlee/ns/dqa#hasQualityRequiredModel">
        <rdfs:domain rdf:resource="http://local.tamu.edu/djlee/ns/dqa#InformationProduct"/>
        <rdfs:range rdf:resource="http://local.tamu.edu/djlee/ns/dqa#Quality_Model_Required"/>
        <rdfs:comment>This property indicates that there are specific required quality levels for an information product.</rdfs:comment>
    </owl:ObjectProperty>
    


    <!-- http://local.tamu.edu/djlee/ns/dqa#hasSource -->

    <owl:ObjectProperty rdf:about="http://local.tamu.edu/djlee/ns/dqa#hasSource">
        <rdfs:domain rdf:resource="http://local.tamu.edu/djlee/ns/dqa#Quality_Problem"/>
        <rdfs:range rdf:resource="http://www.semanticweb.org/djlee/ontologies/2023/8/untitled-ontology-71#Problem_Source"/>
        <rdfs:comment>Connects Problem to Problem Source</rdfs:comment>
    </owl:ObjectProperty>
    


    <!-- http://local.tamu.edu/djlee/ns/dqa#identifierdBy -->

    <owl:ObjectProperty rdf:about="http://local.tamu.edu/djlee/ns/dqa#identifierdBy">
        <rdfs:domain rdf:resource="http://local.tamu.edu/djlee/ns/dqa#Quality_Problem"/>
        <rdfs:range rdf:resource="http://local.tamu.edu/djlee/ns/dqa#Quality_Model_Active"/>
        <rdfs:comment>Specifies that a QualityProblem is identified through specific QualityActiveModel.</rdfs:comment>
    </owl:ObjectProperty>
    


    <!-- http://local.tamu.edu/djlee/ns/dqa#involvedIn -->

    <owl:ObjectProperty rdf:about="http://local.tamu.edu/djlee/ns/dqa#involvedIn">
        <rdfs:domain rdf:resource="https://www.w3.org/TR/prov-o/#Activity"/>
        <rdfs:range rdf:resource="https://www.w3.org/TR/prov-o/#Activity"/>
        <rdfs:comment>Indicate relationships between associated activities.
Example: Agents may have communication between them about certain evaluation activities or their intervention activities.(source: ISO9000&apos;s Continous Improvement)</rdfs:comment>
    </owl:ObjectProperty>
    


    <!-- http://local.tamu.edu/djlee/ns/dqa#isPartOf -->

    <owl:ObjectProperty rdf:about="http://local.tamu.edu/djlee/ns/dqa#isPartOf">
        <skos:definition>Indicate A is partial components of B (Source: OWL)</skos:definition>
    </owl:ObjectProperty>
    


    <!-- http://local.tamu.edu/djlee/ns/dqa#requiresExpertise -->

    <owl:ObjectProperty rdf:about="http://local.tamu.edu/djlee/ns/dqa#requiresExpertise">
        <rdfs:domain rdf:resource="http://local.tamu.edu/djlee/ns/dqa#InformationProduct"/>
        <rdfs:range rdf:resource="https://www.w3.org/TR/prov-o/#Agent"/>
        <skos:definition>Indicates information product requires domain expertise or skillset of Agents (source: IQAF)</skos:definition>
    </owl:ObjectProperty>
    


    <!-- http://local.tamu.edu/djlee/ns/dqa#verifies -->

    <owl:ObjectProperty rdf:about="http://local.tamu.edu/djlee/ns/dqa#verifies">
        <rdfs:domain rdf:resource="http://local.tamu.edu/djlee/ns/dqa#Quality_Model_Active"/>
        <rdfs:range rdf:resource="http://local.tamu.edu/djlee/ns/dqa#Quality_Model_Required"/>
        <rdfs:comment>Establishes that the QualityActiveModel verifies compliance with a Quality Required Model.</rdfs:comment>
    </owl:ObjectProperty>
    


    <!-- http://www.semanticweb.org/djlee/ontologies/2023/8/untitled-ontology-71#affectsActivities -->

    <owl:ObjectProperty rdf:about="http://www.semanticweb.org/djlee/ontologies/2023/8/untitled-ontology-71#affectsActivities">
        <rdfs:domain rdf:resource="http://www.semanticweb.org/djlee/ontologies/2023/8/untitled-ontology-71#Problem_Source"/>
        <rdfs:range rdf:resource="http://www.semanticweb.org/djlee/ontologies/2023/8/untitled-ontology-71#Activity_Type"/>
        <skos:definition>Relationship between data quality problem source and activity types
(IQAF, https://doi.org/10.1002/asi.20652)</skos:definition>
    </owl:ObjectProperty>
    


    <!-- http://www.semanticweb.org/djlee/ontologies/2023/8/untitled-ontology-71#affectsDimensions -->

    <owl:ObjectProperty rdf:about="http://www.semanticweb.org/djlee/ontologies/2023/8/untitled-ontology-71#affectsDimensions">
        <rdfs:domain rdf:resource="http://www.semanticweb.org/djlee/ontologies/2023/8/untitled-ontology-71#Problem_Source"/>
        <rdfs:range rdf:resource="http://www.w3.org/ns/dqv#Dimension"/>
        <skos:definition>Relationship between data quality problem source and quality dimensions.
(IQAF, https://doi.org/10.1002/asi.20652)</skos:definition>
    </owl:ObjectProperty>
    


    <!-- http://www.semanticweb.org/djlee/ontologies/2023/8/untitled-ontology-71#composedOf -->

    <owl:ObjectProperty rdf:about="http://www.semanticweb.org/djlee/ontologies/2023/8/untitled-ontology-71#composedOf">
        <rdfs:domain rdf:resource="https://www.w3.org/TR/prov-o/#Activity"/>
        <rdfs:range rdf:resource="http://www.semanticweb.org/djlee/ontologies/2023/8/untitled-ontology-71#Action"/>
        <skos:definition>Indicates A is composed of B (Source: iso 9000)</skos:definition>
    </owl:ObjectProperty>
    


    <!-- http://www.semanticweb.org/djlee/ontologies/2023/8/untitled-ontology-71#comprisedOf -->

    <owl:ObjectProperty rdf:about="http://www.semanticweb.org/djlee/ontologies/2023/8/untitled-ontology-71#comprisedOf">
        <skos:definition>Specifying something physically contained by something else. Typically used here for the underlying anatomical structures, such as organs, that comprise the anatomical system.
(source: Schema.org)</skos:definition>
    </owl:ObjectProperty>
    


    <!-- http://www.semanticweb.org/djlee/ontologies/2023/8/untitled-ontology-71#curates -->

    <owl:ObjectProperty rdf:about="http://www.semanticweb.org/djlee/ontologies/2023/8/untitled-ontology-71#curates">
        <rdfs:domain rdf:resource="https://www.w3.org/TR/prov-o/#Person"/>
        <rdfs:range rdf:resource="http://local.tamu.edu/djlee/ns/dqa#InformationProduct"/>
        <skos:definition>Indicate A is curator of B
(source: Schema.org, DDI)</skos:definition>
    </owl:ObjectProperty>
    


    <!-- http://www.semanticweb.org/djlee/ontologies/2023/8/untitled-ontology-71#evaluateDQA -->

    <owl:ObjectProperty rdf:about="http://www.semanticweb.org/djlee/ontologies/2023/8/untitled-ontology-71#evaluateDQA">
        <rdfs:domain rdf:resource="http://www.semanticweb.org/djlee/ontologies/2023/8/untitled-ontology-71#DQA_Process_Improvement"/>
        <rdfs:range rdf:resource="http://www.semanticweb.org/djlee/ontologies/2023/8/untitled-ontology-71#DQA_Evaluation"/>
        <rdfs:comment>connects the process of DQA Process Improvement to DQA Process Evaluation Activity</rdfs:comment>
    </owl:ObjectProperty>
    


    <!-- http://www.semanticweb.org/djlee/ontologies/2023/8/untitled-ontology-71#intervenesInDQA -->

    <owl:ObjectProperty rdf:about="http://www.semanticweb.org/djlee/ontologies/2023/8/untitled-ontology-71#intervenesInDQA">
        <rdfs:domain rdf:resource="http://www.semanticweb.org/djlee/ontologies/2023/8/untitled-ontology-71#DQA_Process_Improvement"/>
        <rdfs:range rdf:resource="http://www.semanticweb.org/djlee/ontologies/2023/8/untitled-ontology-71#DQA_Intervention"/>
        <rdfs:comment>Connects a DQA process to activities aimed at its improvement.</rdfs:comment>
    </owl:ObjectProperty>
    


    <!-- http://www.semanticweb.org/djlee/ontologies/2023/8/untitled-ontology-71#involvesCommunication -->

    <owl:ObjectProperty rdf:about="http://www.semanticweb.org/djlee/ontologies/2023/8/untitled-ontology-71#involvesCommunication">
        <rdfs:domain rdf:resource="http://www.semanticweb.org/djlee/ontologies/2023/8/untitled-ontology-71#DQA_Process"/>
        <rdfs:range rdf:resource="http://local.tamu.edu/djlee/ns/dqa#Communication"/>
        <rdfs:comment>Links the DQA process to its communication activities, emphasizing the importance of documentation and discussion in quality assurance.</rdfs:comment>
    </owl:ObjectProperty>
    


    <!-- http://www.semanticweb.org/djlee/ontologies/2023/8/untitled-ontology-71#involvesEvaluation -->

    <owl:ObjectProperty rdf:about="http://www.semanticweb.org/djlee/ontologies/2023/8/untitled-ontology-71#involvesEvaluation">
        <rdfs:subPropertyOf rdf:resource="http://www.w3.org/2002/07/owl#topObjectProperty"/>
        <rdfs:domain rdf:resource="http://www.semanticweb.org/djlee/ontologies/2023/8/untitled-ontology-71#DQA_Process"/>
        <rdfs:range rdf:resource="http://www.semanticweb.org/djlee/ontologies/2023/8/untitled-ontology-71#Evaluation"/>
        <rdfs:comment>Indicates that the DQA process involves a systematic evaluation of data products.</rdfs:comment>
    </owl:ObjectProperty>
    


    <!-- http://www.semanticweb.org/djlee/ontologies/2023/8/untitled-ontology-71#involvesIntervention -->

    <owl:ObjectProperty rdf:about="http://www.semanticweb.org/djlee/ontologies/2023/8/untitled-ontology-71#involvesIntervention">
        <rdfs:domain rdf:resource="http://www.semanticweb.org/djlee/ontologies/2023/8/untitled-ontology-71#DQA_Process"/>
        <rdfs:range rdf:resource="http://local.tamu.edu/djlee/ns/dqa#Intervention"/>
        <rdfs:comment>Connects the DQA process to interventions that arise from the evaluation activities.</rdfs:comment>
    </owl:ObjectProperty>
    


    <!-- http://www.semanticweb.org/djlee/ontologies/2023/8/untitled-ontology-71#isDescribedBy -->

    <owl:ObjectProperty rdf:about="http://www.semanticweb.org/djlee/ontologies/2023/8/untitled-ontology-71#isDescribedBy">
        <rdfs:domain rdf:resource="http://local.tamu.edu/djlee/ns/dqa#Data"/>
        <rdfs:range rdf:resource="http://local.tamu.edu/djlee/ns/dqa#Metadata"/>
        <rdfs:comment>A data product is described by the associated metadata product.</rdfs:comment>
    </owl:ObjectProperty>
    


    <!-- http://www.semanticweb.org/djlee/ontologies/2023/8/untitled-ontology-71#isMeasuredBy -->

    <owl:ObjectProperty rdf:about="http://www.semanticweb.org/djlee/ontologies/2023/8/untitled-ontology-71#isMeasuredBy">
        <rdfs:domain rdf:resource="http://www.w3.org/ns/dqv#Dimension"/>
        <rdfs:range rdf:resource="http://www.w3.org/ns/dqv#Metric"/>
        <rdfs:comment>This is an object propert that connects dimensions to metrics. In particular, a demension is measured by a specific metric(s).</rdfs:comment>
    </owl:ObjectProperty>
    


    <!-- http://www.semanticweb.org/djlee/ontologies/2023/8/untitled-ontology-71#isMediatedBy -->

    <owl:ObjectProperty rdf:about="http://www.semanticweb.org/djlee/ontologies/2023/8/untitled-ontology-71#isMediatedBy">
        <rdfs:domain rdf:resource="https://www.w3.org/TR/prov-o/#Activity"/>
        <skos:definition>Indicates DQA activities are mediated by different types of tools. (Source: Activity Theory)</skos:definition>
    </owl:ObjectProperty>
    


    <!-- http://www.semanticweb.org/djlee/ontologies/2023/8/untitled-ontology-71#isPerformedBy -->

    <owl:ObjectProperty rdf:about="http://www.semanticweb.org/djlee/ontologies/2023/8/untitled-ontology-71#isPerformedBy">
        <rdfs:domain rdf:resource="https://www.w3.org/TR/prov-o/#Activity"/>
        <rdfs:range rdf:resource="https://www.w3.org/TR/prov-o/#Agent"/>
        <skos:definition>Indicate agents&apos; contribution to DQA activities (source: Activity Theory)</skos:definition>
    </owl:ObjectProperty>
    


    <!-- http://www.semanticweb.org/djlee/ontologies/2023/8/untitled-ontology-71#mediates -->

    <owl:ObjectProperty rdf:about="http://www.semanticweb.org/djlee/ontologies/2023/8/untitled-ontology-71#mediates">
        <rdfs:domain rdf:resource="https://www.w3.org/TR/prov-o/#Agent"/>
        <skos:definition>Of a person or other agency: to act as a mediator or intermediary; to intercede or intervene. In later use chiefly with between.(source: Activity Theory)</skos:definition>
    </owl:ObjectProperty>
    


    <!-- http://www.semanticweb.org/djlee/ontologies/2023/8/untitled-ontology-71#playRole -->

    <owl:ObjectProperty rdf:about="http://www.semanticweb.org/djlee/ontologies/2023/8/untitled-ontology-71#playRole">
        <rdfs:subPropertyOf rdf:resource="http://www.w3.org/2002/07/owl#topObjectProperty"/>
        <rdfs:domain rdf:resource="https://www.w3.org/TR/prov-o/#Agent"/>
        <rdfs:range rdf:resource="http://local.tamu.edu/djlee/ns/dqa#Role"/>
        <skos:definition>A role is the function of an  agent with respect to an activity, in the context of a usage, generation, invalidation, association, start, and end. (Source: PROV Ontology)</skos:definition>
    </owl:ObjectProperty>
    


    <!-- http://www.semanticweb.org/djlee/ontologies/2023/8/untitled-ontology-71#provides -->

    <owl:ObjectProperty rdf:about="http://www.semanticweb.org/djlee/ontologies/2023/8/untitled-ontology-71#provides">
        <rdfs:domain rdf:resource="https://www.w3.org/TR/prov-o/#Agent"/>
        <rdfs:range rdf:resource="http://local.tamu.edu/djlee/ns/dqa#InformationProduct"/>
        <skos:definition>Indicates the source of information products (source: Schema.org)</skos:definition>
    </owl:ObjectProperty>
    


    <!-- http://www.semanticweb.org/djlee/ontologies/2023/8/untitled-ontology-71#targets -->

    <owl:ObjectProperty rdf:about="http://www.semanticweb.org/djlee/ontologies/2023/8/untitled-ontology-71#targets">
        <skos:definition>The relationship between an action and its Target. (source: Web Annotation Voca.)</skos:definition>
    </owl:ObjectProperty>
    


    <!-- http://www.semanticweb.org/djlee/ontologies/2023/8/untitled-ontology-71#usedIn -->

    <owl:ObjectProperty rdf:about="http://www.semanticweb.org/djlee/ontologies/2023/8/untitled-ontology-71#usedIn">
        <rdfs:domain rdf:resource="http://www.semanticweb.org/djlee/ontologies/2023/8/untitled-ontology-71#Method"/>
        <rdfs:range rdf:resource="https://www.w3.org/TR/prov-o/#Activity"/>
        <skos:definition>Usage in &quot;usedIn&quot; is the beginning of utilizing a method by an activity. (Source: PROV Ontology)</skos:definition>
    </owl:ObjectProperty>
    


    <!-- http://www.w3.org/TR/prov-o#isAttributedTo -->

    <owl:ObjectProperty rdf:about="http://www.w3.org/TR/prov-o#isAttributedTo">
        <owl:equivalentProperty rdf:resource="http://www.w3.org/TR/prov-o#isDerivedFrom"/>
        <rdfs:domain rdf:resource="http://local.tamu.edu/djlee/ns/dqa#InformationProduct"/>
        <skos:definition>Attribution is the ascribing of an entity to an agent.

(source: PROV Ontology)</skos:definition>
    </owl:ObjectProperty>
    


    <!-- http://www.w3.org/TR/prov-o#isDerivedFrom -->

    <owl:ObjectProperty rdf:about="http://www.w3.org/TR/prov-o#isDerivedFrom">
        <owl:equivalentProperty rdf:resource="http://www.w3.org/TR/prov-o#isGeneratedBy"/>
        <rdfs:domain rdf:resource="http://local.tamu.edu/djlee/ns/dqa#InformationProduct"/>
        <skos:definition>A derivation is a transformation of an entity into another, an update of an entity resulting in a new one, or the construction of a new entity based on a pre-existing entity.

(source: PROV Ontology)</skos:definition>
    </owl:ObjectProperty>
    


    <!-- http://www.w3.org/TR/prov-o#isGeneratedBy -->

    <owl:ObjectProperty rdf:about="http://www.w3.org/TR/prov-o#isGeneratedBy">
        <rdfs:domain rdf:resource="http://local.tamu.edu/djlee/ns/dqa#InformationProduct"/>
        <skos:definition>Generation is the completion of production of a new entity by an activity. This entity did not exist before generation and becomes available for usage after this generation.

(Source: PROV Ontology)</skos:definition>
    </owl:ObjectProperty>
    


    <!-- http://www.w3.org/ns/dqv#isMeasurementOf -->

    <owl:ObjectProperty rdf:about="http://www.w3.org/ns/dqv#isMeasurementOf">
        <rdfs:domain rdf:resource="http://www.semanticweb.org/djlee/ontologies/2023/8/untitled-ontology-71#Quality_Measurement"/>
        <rdfs:range rdf:resource="http://www.w3.org/ns/dqv#Metric"/>
        <skos:definition>Indicates the metric being observed.
(Source: DQV)</skos:definition>
    </owl:ObjectProperty>
    


    <!-- http://www.w3.org/ns/oa#motivatedBy -->

    <owl:ObjectProperty rdf:about="http://www.w3.org/ns/oa#motivatedBy">
        <rdfs:domain rdf:resource="https://www.w3.org/TR/prov-o/#Activity"/>
        <rdfs:range rdf:resource="http://www.semanticweb.org/djlee/ontologies/2023/8/untitled-ontology-71#Objective"/>
        <skos:definition>The relationship between an Annotation and a Motivation that describes the reason for the Annotation&apos;s creation.

(Web Annotation Voca.)</skos:definition>
    </owl:ObjectProperty>
    


    <!-- https://www.w3.org/TR/prov-o/#actedOnBehalfOf -->

    <owl:ObjectProperty rdf:about="https://www.w3.org/TR/prov-o/#actedOnBehalfOf">
        <rdfs:domain rdf:resource="https://www.w3.org/TR/prov-o/#Agent"/>
        <rdfs:range rdf:resource="https://www.w3.org/TR/prov-o/#Agent"/>
        <skos:definition>Delegation is the assignment of authority and responsibility to an agent (by itself or by another agent) to carry out a specific activity as a delegate or representative, while the agent it acts on behalf of retains some responsibility for the outcome of the delegated work. For example, a student acted on behalf of his supervisor, who acted on behalf of the department chair, who acted on behalf of the university; all those agents are responsible in some way for the activity that took place but we do not say explicitly who bears responsibility and to what degree.

(PROV Ontology)</skos:definition>
    </owl:ObjectProperty>
    


    <!-- https://www.w3.org/TR/prov-o/#allocatedBy -->

    <owl:ObjectProperty rdf:about="https://www.w3.org/TR/prov-o/#allocatedBy">
        <rdfs:domain rdf:resource="http://local.tamu.edu/djlee/ns/dqa#Role"/>
        <rdfs:range rdf:resource="http://local.tamu.edu/djlee/ns/dqa#DivisionOfLabor"/>
        <rdfs:comment>AllocatedBy is the assignment of authority and responsibility to a role of agents to carry out a specific activity as a representative.

(Source: prov:qualifiedDelegation, PROV Ontology)</rdfs:comment>
    </owl:ObjectProperty>
    


    <!-- https://www.w3.org/TR/prov-o/#hasPrimarySource -->

    <owl:ObjectProperty rdf:about="https://www.w3.org/TR/prov-o/#hasPrimarySource">
        <rdfs:domain rdf:resource="https://www.w3.org/TR/prov-o/#Agent"/>
        <skos:definition>A primary source for a topic refers to something produced by some agent with direct experience and knowledge about the topic, at the time of the topic&apos;s study, without benefit from hindsight. Because of the directness of primary sources, they &apos;speak for themselves&apos; in ways that cannot be captured through the filter of secondary sources. As such, it is important for secondary sources to reference those primary sources from which they were derived, so that their reliability can be investigated. A primary source relation is a particular case of derivation of secondary materials from their primary sources. It is recognized that the determination of primary sources can be up to interpretation, and should be done according to conventions accepted within the application&apos;s domain.

(sourec: PROV Ontology, WebAnnotation)</skos:definition>
    </owl:ObjectProperty>
    


    <!-- https://www.w3.org/TR/prov-o/#isAssociatedWith -->

    <owl:ObjectProperty rdf:about="https://www.w3.org/TR/prov-o/#isAssociatedWith">
        <rdfs:domain rdf:resource="http://local.tamu.edu/djlee/ns/dqa#ProfessionalDevelopment"/>
        <rdfs:range rdf:resource="http://www.semanticweb.org/djlee/ontologies/2023/8/untitled-ontology-71#Group"/>
        <skos:definition>An activity association is an assignment of responsibility to an agent for an activity, indicating that the agent had a role in the activity. It further allows for a plan to be specified, which is the plan intended by the agent to achieve some goals in the context of this activity.

(source: PROV Ontology)</skos:definition>
    </owl:ObjectProperty>
    


    <!-- https://www.w3.org/TR/prov-o/#used -->

    <owl:ObjectProperty rdf:about="https://www.w3.org/TR/prov-o/#used">
        <rdfs:domain rdf:resource="https://www.w3.org/TR/prov-o/#Agent"/>
        <rdfs:range rdf:resource="http://local.tamu.edu/djlee/ns/dqa#InformationProduct"/>
        <skos:definition>Usage is the beginning of utilizing an entity by an activity. Before usage, the activity had not begun to utilize this entity and could not have been affected by the entity.

(source: PROV Ontology)</skos:definition>
    </owl:ObjectProperty>
    


    <!-- https://www.w3.org/TR/vocab-duv/#hasDistributor -->

    <owl:ObjectProperty rdf:about="https://www.w3.org/TR/vocab-duv/#hasDistributor">
        <rdfs:domain rdf:resource="http://local.tamu.edu/djlee/ns/dqa#InformationProduct"/>
        <rdfs:range rdf:resource="https://www.w3.org/TR/prov-o/#Agent"/>
        <skos:definition>The distributor is the organization that makes the dataset or distribution available for downloading and use.
(source: Dataset Usage Vocabulary)</skos:definition>
    </owl:ObjectProperty>
    


    <!-- https://www.w3.org/TR/vocab-duv/#hasFeedback -->

    <owl:ObjectProperty rdf:about="https://www.w3.org/TR/vocab-duv/#hasFeedback">
        <rdfs:domain rdf:resource="https://www.w3.org/TR/prov-o/#Agent"/>
        <rdfs:range rdf:resource="http://www.w3.org/ns/dqv#UserQualityFeedback"/>
        <skos:definition>Agents provide feedback about data quality (source: Dataset Usage Voca.)</skos:definition>
    </owl:ObjectProperty>
    


    <!-- https://www.w3.org/TR/vocab-duv/#refersTo -->

    <owl:ObjectProperty rdf:about="https://www.w3.org/TR/vocab-duv/#refersTo">
        <rdfs:domain rdf:resource="http://www.w3.org/ns/dqv#Metric"/>
        <rdfs:range rdf:resource="http://local.tamu.edu/djlee/ns/dqa#ReferenceSource"/>
        <skos:definition>Dataset/distribution associated with Usage.
(Source: Dataset Usage Voca.)</skos:definition>
    </owl:ObjectProperty>
    


    <!-- 
    ///////////////////////////////////////////////////////////////////////////////////////
    //
    // Data properties
    //
    ///////////////////////////////////////////////////////////////////////////////////////
     -->

    


    <!-- http://local.tamu.edu/djlee/ns/dqa#qualityMeasurementValue -->

    <owl:DatatypeProperty rdf:about="http://local.tamu.edu/djlee/ns/dqa#qualityMeasurementValue">
        <skos:definition>This property contains a value of a particular measurement.</skos:definition>
    </owl:DatatypeProperty>
    


    <!-- http://local.tamu.edu/djlee/ns/dqa#qualityMeasurementValueRequired -->

    <owl:DatatypeProperty rdf:about="http://local.tamu.edu/djlee/ns/dqa#qualityMeasurementValueRequired">
        <rdfs:domain rdf:resource="http://www.semanticweb.org/djlee/ontologies/2023/8/untitled-ontology-71#Quality_Measurement"/>
        <rdfs:comment>This property contains a value indicating the required level quality of a particular measurement.</rdfs:comment>
    </owl:DatatypeProperty>
    


    <!-- http://www.semanticweb.org/djlee/ontologies/2023/8/untitled-ontology-71#availableFunding -->

    <owl:DatatypeProperty rdf:about="http://www.semanticweb.org/djlee/ontologies/2023/8/untitled-ontology-71#availableFunding">
        <rdfs:domain rdf:resource="http://local.tamu.edu/djlee/ns/dqa#InformationProduct"/>
        <rdfs:range rdf:resource="http://www.w3.org/2001/XMLSchema#float"/>
        <skos:definition>Describe funding source of information product if available.</skos:definition>
    </owl:DatatypeProperty>
    


    <!-- http://www.semanticweb.org/djlee/ontologies/2023/8/untitled-ontology-71#cost -->

    <owl:DatatypeProperty rdf:about="http://www.semanticweb.org/djlee/ontologies/2023/8/untitled-ontology-71#cost">
        <rdfs:domain rdf:resource="http://local.tamu.edu/djlee/ns/dqa#InformationProduct"/>
        <rdfs:range rdf:resource="http://www.w3.org/2001/XMLSchema#float"/>
        <skos:definition>Any cost involved in the information products</skos:definition>
    </owl:DatatypeProperty>
    


    <!-- http://www.semanticweb.org/djlee/ontologies/2023/8/untitled-ontology-71#criticalityValue -->

    <owl:DatatypeProperty rdf:about="http://www.semanticweb.org/djlee/ontologies/2023/8/untitled-ontology-71#criticalityValue">
        <rdfs:domain rdf:resource="http://local.tamu.edu/djlee/ns/dqa#InformationProduct"/>
        <rdfs:range rdf:resource="http://www.w3.org/2001/XMLSchema#float"/>
        <rdfs:comment>Contains a number indicating the relative value of a dataset to RDR</rdfs:comment>
    </owl:DatatypeProperty>
    


    <!-- http://www.semanticweb.org/djlee/ontologies/2023/8/untitled-ontology-71#currentQuality -->

    <owl:DatatypeProperty rdf:about="http://www.semanticweb.org/djlee/ontologies/2023/8/untitled-ontology-71#currentQuality">
        <rdfs:domain rdf:resource="http://local.tamu.edu/djlee/ns/dqa#InformationProduct"/>
        <rdfs:range rdf:resource="http://www.w3.org/2001/XMLSchema#float"/>
        <skos:definition>Note of current quality level or score of information product based on its evaluation</skos:definition>
    </owl:DatatypeProperty>
    


    <!-- http://www.semanticweb.org/djlee/ontologies/2023/8/untitled-ontology-71#priority -->

    <owl:DatatypeProperty rdf:about="http://www.semanticweb.org/djlee/ontologies/2023/8/untitled-ontology-71#priority">
        <rdfs:domain rdf:resource="http://local.tamu.edu/djlee/ns/dqa#InformationProduct"/>
        <rdfs:range rdf:resource="http://www.w3.org/2001/XMLSchema#float"/>
        <rdfs:comment>Contains the ovarall criticality score for dataset based on its criticality value, available funding, cost, current quality, and available expertise.</rdfs:comment>
    </owl:DatatypeProperty>
    


    <!-- 
    ///////////////////////////////////////////////////////////////////////////////////////
    //
    // Classes
    //
    ///////////////////////////////////////////////////////////////////////////////////////
     -->

    


    <!-- http://local.tamu.edu/djlee/ns/dqa#Add -->

    <owl:Class rdf:about="http://local.tamu.edu/djlee/ns/dqa#Add">
        <owl:equivalentClass>
            <owl:Restriction>
                <owl:onProperty rdf:resource="http://www.semanticweb.org/djlee/ontologies/2023/8/untitled-ontology-71#targets"/>
                <owl:someValuesFrom rdf:resource="http://local.tamu.edu/djlee/ns/dqa#InformationProduct"/>
            </owl:Restriction>
        </owl:equivalentClass>
        <rdfs:subClassOf rdf:resource="http://www.semanticweb.org/djlee/ontologies/2023/8/untitled-ontology-71#Action"/>
        <skos:definition>The act of editing by adding an object to a collection.
(Schema.org)</skos:definition>
    </owl:Class>
    


    <!-- http://local.tamu.edu/djlee/ns/dqa#ApprovalReview -->

    <owl:Class rdf:about="http://local.tamu.edu/djlee/ns/dqa#ApprovalReview">
        <rdfs:subClassOf rdf:resource="http://www.w3.org/ns/dqv#QualityCertificate"/>
        <rdfs:isDefinedBy>DDI</rdfs:isDefinedBy>
        <skos:definition>Provides information about the Approval Review undertaken in relation to the activity. Identifies the organization processing the review, the role of the approval review organization, case number, description, and related dates. Allows the inclusion of a reference to an external source detailing the approval review.</skos:definition>
    </owl:Class>
    


    <!-- http://local.tamu.edu/djlee/ns/dqa#CharacteristicData -->

    <owl:Class rdf:about="http://local.tamu.edu/djlee/ns/dqa#CharacteristicData">
        <rdfs:subClassOf rdf:resource="http://local.tamu.edu/djlee/ns/dqa#QualityStatement"/>
        <rdfs:isDefinedBy>iso 8000</rdfs:isDefinedBy>
        <skos:definition>description of an entity by the class to which it belongs and a set of property values</skos:definition>
    </owl:Class>
    


    <!-- http://local.tamu.edu/djlee/ns/dqa#Communication -->

    <owl:Class rdf:about="http://local.tamu.edu/djlee/ns/dqa#Communication">
        <owl:equivalentClass>
            <owl:Restriction>
                <owl:onProperty rdf:resource="http://local.tamu.edu/djlee/ns/dqa#involvedIn"/>
                <owl:someValuesFrom rdf:resource="http://local.tamu.edu/djlee/ns/dqa#Intervention"/>
            </owl:Restriction>
        </owl:equivalentClass>
        <owl:equivalentClass>
            <owl:Restriction>
                <owl:onProperty rdf:resource="http://local.tamu.edu/djlee/ns/dqa#involvedIn"/>
                <owl:someValuesFrom rdf:resource="http://www.semanticweb.org/djlee/ontologies/2023/8/untitled-ontology-71#Evaluation"/>
            </owl:Restriction>
        </owl:equivalentClass>
        <owl:equivalentClass>
            <owl:Restriction>
                <owl:onProperty rdf:resource="http://www.semanticweb.org/djlee/ontologies/2023/8/untitled-ontology-71#composedOf"/>
                <owl:someValuesFrom rdf:resource="http://www.semanticweb.org/djlee/ontologies/2023/8/untitled-ontology-71#Ask"/>
            </owl:Restriction>
        </owl:equivalentClass>
        <owl:equivalentClass>
            <owl:Restriction>
                <owl:onProperty rdf:resource="http://www.semanticweb.org/djlee/ontologies/2023/8/untitled-ontology-71#composedOf"/>
                <owl:someValuesFrom rdf:resource="http://www.semanticweb.org/djlee/ontologies/2023/8/untitled-ontology-71#Ask_permission_to_intervene"/>
            </owl:Restriction>
        </owl:equivalentClass>
        <owl:equivalentClass>
            <owl:Restriction>
                <owl:onProperty rdf:resource="http://www.semanticweb.org/djlee/ontologies/2023/8/untitled-ontology-71#composedOf"/>
                <owl:someValuesFrom rdf:resource="http://www.semanticweb.org/djlee/ontologies/2023/8/untitled-ontology-71#Comment"/>
            </owl:Restriction>
        </owl:equivalentClass>
        <owl:equivalentClass>
            <owl:Restriction>
                <owl:onProperty rdf:resource="http://www.semanticweb.org/djlee/ontologies/2023/8/untitled-ontology-71#composedOf"/>
                <owl:someValuesFrom rdf:resource="http://www.semanticweb.org/djlee/ontologies/2023/8/untitled-ontology-71#Confirm"/>
            </owl:Restriction>
        </owl:equivalentClass>
        <owl:equivalentClass>
            <owl:Restriction>
                <owl:onProperty rdf:resource="http://www.semanticweb.org/djlee/ontologies/2023/8/untitled-ontology-71#composedOf"/>
                <owl:someValuesFrom rdf:resource="http://www.semanticweb.org/djlee/ontologies/2023/8/untitled-ontology-71#Inform"/>
            </owl:Restriction>
        </owl:equivalentClass>
        <owl:equivalentClass>
            <owl:Restriction>
                <owl:onProperty rdf:resource="http://www.semanticweb.org/djlee/ontologies/2023/8/untitled-ontology-71#composedOf"/>
                <owl:someValuesFrom rdf:resource="http://www.semanticweb.org/djlee/ontologies/2023/8/untitled-ontology-71#Interact"/>
            </owl:Restriction>
        </owl:equivalentClass>
        <owl:equivalentClass>
            <owl:Restriction>
                <owl:onProperty rdf:resource="http://www.semanticweb.org/djlee/ontologies/2023/8/untitled-ontology-71#composedOf"/>
                <owl:someValuesFrom rdf:resource="http://www.semanticweb.org/djlee/ontologies/2023/8/untitled-ontology-71#Release"/>
            </owl:Restriction>
        </owl:equivalentClass>
        <owl:equivalentClass>
            <owl:Restriction>
                <owl:onProperty rdf:resource="http://www.semanticweb.org/djlee/ontologies/2023/8/untitled-ontology-71#composedOf"/>
                <owl:someValuesFrom rdf:resource="http://www.semanticweb.org/djlee/ontologies/2023/8/untitled-ontology-71#Share"/>
            </owl:Restriction>
        </owl:equivalentClass>
        <owl:equivalentClass>
            <owl:Restriction>
                <owl:onProperty rdf:resource="http://www.w3.org/ns/oa#motivatedBy"/>
                <owl:someValuesFrom rdf:resource="http://local.tamu.edu/djlee/ns/dqa#Quality_Objective"/>
            </owl:Restriction>
        </owl:equivalentClass>
        <rdfs:subClassOf rdf:resource="https://www.w3.org/TR/prov-o/#Activity"/>
        <rdfs:comment>Communication class describes DQA communication activity. 
Agent performs Communication activity to share information about and coordinate Evaluation and Intervention activities using communication Actions.</rdfs:comment>
    </owl:Class>
    


    <!-- http://local.tamu.edu/djlee/ns/dqa#Community -->

    <owl:Class rdf:about="http://local.tamu.edu/djlee/ns/dqa#Community">
        <rdfs:subClassOf rdf:resource="http://www.semanticweb.org/djlee/ontologies/2023/8/untitled-ontology-71#Group"/>
        <rdfs:comment>Used to describe the Agent type Community</rdfs:comment>
    </owl:Class>
    


    <!-- http://local.tamu.edu/djlee/ns/dqa#Complaint -->

    <owl:Class rdf:about="http://local.tamu.edu/djlee/ns/dqa#Complaint">
        <rdfs:subClassOf rdf:resource="http://www.w3.org/ns/dqv#QualityAnnotation"/>
        <rdfs:isDefinedBy>iso 9000</rdfs:isDefinedBy>
        <skos:definition>&lt;customer satisfaction&gt; expression of dissatisfaction made to an organization (3.2.1), related to its product (3.7.6) or service (3.7.7), or the complaints-handling process (3.4.1) itself, where a response or resolution is explicitly or implicitly expected</skos:definition>
    </owl:Class>
    


    <!-- http://local.tamu.edu/djlee/ns/dqa#ComplianceStatement -->

    <owl:Class rdf:about="http://local.tamu.edu/djlee/ns/dqa#ComplianceStatement">
        <rdfs:subClassOf rdf:resource="http://local.tamu.edu/djlee/ns/dqa#ReferenceSource"/>
        <rdfs:isDefinedBy>Data Documentation Initiative</rdfs:isDefinedBy>
        <skos:definition>Describe the measures taken to comply with the standards and/or specific levels of compliance by providing further details or a general description of compliance with the standard.</skos:definition>
    </owl:Class>
    


    <!-- http://local.tamu.edu/djlee/ns/dqa#ConformanceResult -->

    <owl:Class rdf:about="http://local.tamu.edu/djlee/ns/dqa#ConformanceResult">
        <rdfs:subClassOf rdf:resource="http://local.tamu.edu/djlee/ns/dqa#DataQuality"/>
        <rdfs:subClassOf rdf:resource="http://local.tamu.edu/djlee/ns/dqa#MetadataQuality"/>
        <rdfs:isDefinedBy>iso 19157</rdfs:isDefinedBy>
        <skos:definition>Results of conformance (fulfilment of specified requirements)</skos:definition>
    </owl:Class>
    


    <!-- http://local.tamu.edu/djlee/ns/dqa#Correction -->

    <owl:Class rdf:about="http://local.tamu.edu/djlee/ns/dqa#Correction">
        <owl:equivalentClass>
            <owl:Restriction>
                <owl:onProperty rdf:resource="http://www.semanticweb.org/djlee/ontologies/2023/8/untitled-ontology-71#targets"/>
                <owl:someValuesFrom rdf:resource="http://www.semanticweb.org/djlee/ontologies/2023/8/untitled-ontology-71#Creation"/>
            </owl:Restriction>
        </owl:equivalentClass>
        <rdfs:subClassOf rdf:resource="http://www.semanticweb.org/djlee/ontologies/2023/8/untitled-ontology-71#Action"/>
        <rdfs:comment>Equivalent to:
DDI:ErrorCorrection
EIA:ErrorCorrection</rdfs:comment>
        <skos:definition>ISO9000: 
Action to eliminate a detected nonconformity</skos:definition>
    </owl:Class>
    


    <!-- http://local.tamu.edu/djlee/ns/dqa#CorrectiveAction -->

    <owl:Class rdf:about="http://local.tamu.edu/djlee/ns/dqa#CorrectiveAction">
        <owl:equivalentClass>
            <owl:Restriction>
                <owl:onProperty rdf:resource="http://www.semanticweb.org/djlee/ontologies/2023/8/untitled-ontology-71#targets"/>
                <owl:someValuesFrom rdf:resource="http://www.semanticweb.org/djlee/ontologies/2023/8/untitled-ontology-71#Creation"/>
            </owl:Restriction>
        </owl:equivalentClass>
        <rdfs:subClassOf rdf:resource="http://www.semanticweb.org/djlee/ontologies/2023/8/untitled-ontology-71#Action"/>
        <skos:definition>ISO9000:
Action to eliminate the cause of a nonconformity and to prevent recurrence</skos:definition>
    </owl:Class>
    


    <!-- http://local.tamu.edu/djlee/ns/dqa#Curator -->

    <owl:Class rdf:about="http://local.tamu.edu/djlee/ns/dqa#Curator">
        <owl:equivalentClass>
            <owl:Restriction>
                <owl:onProperty rdf:resource="http://www.semanticweb.org/djlee/ontologies/2023/8/untitled-ontology-71#curates"/>
                <owl:someValuesFrom rdf:resource="http://local.tamu.edu/djlee/ns/dqa#InformationProduct"/>
            </owl:Restriction>
        </owl:equivalentClass>
        <owl:equivalentClass>
            <owl:Restriction>
                <owl:onProperty rdf:resource="https://www.w3.org/TR/prov-o/#actedOnBehalfOf"/>
                <owl:someValuesFrom rdf:resource="https://www.w3.org/TR/prov-o/#Agent"/>
            </owl:Restriction>
        </owl:equivalentClass>
        <rdfs:subClassOf rdf:resource="https://www.w3.org/TR/prov-o/#Person"/>
        <rdfs:seeAlso>DDI:Evaluator
DDI:ReviewerRole</rdfs:seeAlso>
        <skos:definition>ISO9000
Person who assist the organization on quality management system realization, giving advice or information</skos:definition>
    </owl:Class>
    


    <!-- http://local.tamu.edu/djlee/ns/dqa#CustomerSatisfaction -->

    <owl:Class rdf:about="http://local.tamu.edu/djlee/ns/dqa#CustomerSatisfaction">
        <rdfs:subClassOf rdf:resource="http://www.w3.org/ns/dqv#QualityAnnotation"/>
        <rdfs:isDefinedBy>iso 9000</rdfs:isDefinedBy>
        <skos:definition>customer&apos;s (3.2.4) perception of the degree to which the customer&apos;s expectations have been fulfilled</skos:definition>
    </owl:Class>
    


    <!-- http://local.tamu.edu/djlee/ns/dqa#Data -->

    <owl:Class rdf:about="http://local.tamu.edu/djlee/ns/dqa#Data">
        <owl:equivalentClass>
            <owl:Restriction>
                <owl:onProperty rdf:resource="http://www.semanticweb.org/djlee/ontologies/2023/8/untitled-ontology-71#comprisedOf"/>
                <owl:someValuesFrom rdf:resource="http://www.semanticweb.org/djlee/ontologies/2023/8/untitled-ontology-71#Measurement"/>
            </owl:Restriction>
        </owl:equivalentClass>
        <owl:equivalentClass>
            <owl:Restriction>
                <owl:onProperty rdf:resource="http://www.semanticweb.org/djlee/ontologies/2023/8/untitled-ontology-71#isDescribedBy"/>
                <owl:someValuesFrom rdf:resource="http://local.tamu.edu/djlee/ns/dqa#Metadata"/>
            </owl:Restriction>
        </owl:equivalentClass>
        <rdfs:subClassOf rdf:resource="http://local.tamu.edu/djlee/ns/dqa#InformationProduct"/>
        <rdfs:comment>Described the data part of the data product.</rdfs:comment>
    </owl:Class>
    


    <!-- http://local.tamu.edu/djlee/ns/dqa#DataAccuracyRecord -->

    <owl:Class rdf:about="http://local.tamu.edu/djlee/ns/dqa#DataAccuracyRecord">
        <rdfs:subClassOf rdf:resource="http://local.tamu.edu/djlee/ns/dqa#DataQuality"/>
        <rdfs:isDefinedBy>iso 8000</rdfs:isDefinedBy>
        <skos:definition>record of the information (32.J.) provided about the data accuracy (.3...8.,1Q) of a specified data set (3.Z:4)</skos:definition>
    </owl:Class>
    


    <!-- http://local.tamu.edu/djlee/ns/dqa#DataCompletenessRecord -->

    <owl:Class rdf:about="http://local.tamu.edu/djlee/ns/dqa#DataCompletenessRecord">
        <rdfs:subClassOf rdf:resource="http://local.tamu.edu/djlee/ns/dqa#DataQuality"/>
        <rdfs:isDefinedBy>iso 8000</rdfs:isDefinedBy>
        <skos:definition>record of the information (3.2.1) provided about the data completeness (3.8.12) of a specified data set
(3.2.4)</skos:definition>
    </owl:Class>
    


    <!-- http://local.tamu.edu/djlee/ns/dqa#DataQuality -->

    <owl:Class rdf:about="http://local.tamu.edu/djlee/ns/dqa#DataQuality">
        <rdfs:subClassOf rdf:resource="http://www.w3.org/ns/dqv#QualityAnnotation"/>
        <rdfs:isDefinedBy>iso 8000</rdfs:isDefinedBy>
        <skos:definition>degree to which a set of inherent characteristics of data fulfils requirements</skos:definition>
    </owl:Class>
    


    <!-- http://local.tamu.edu/djlee/ns/dqa#Delete -->

    <owl:Class rdf:about="http://local.tamu.edu/djlee/ns/dqa#Delete">
        <owl:equivalentClass>
            <owl:Restriction>
                <owl:onProperty rdf:resource="http://www.semanticweb.org/djlee/ontologies/2023/8/untitled-ontology-71#targets"/>
                <owl:someValuesFrom rdf:resource="http://local.tamu.edu/djlee/ns/dqa#InformationProduct"/>
            </owl:Restriction>
        </owl:equivalentClass>
        <rdfs:subClassOf rdf:resource="http://www.semanticweb.org/djlee/ontologies/2023/8/untitled-ontology-71#Action"/>
        <skos:definition>The act of editing a recipient by removing one of its objects.
(Schema.org)</skos:definition>
    </owl:Class>
    


    <!-- http://local.tamu.edu/djlee/ns/dqa#Description -->

    <owl:Class rdf:about="http://local.tamu.edu/djlee/ns/dqa#Description">
        <rdfs:subClassOf rdf:resource="http://local.tamu.edu/djlee/ns/dqa#QualityStatement"/>
        <skos:definition>A description of the item.
(Schema.org)</skos:definition>
    </owl:Class>
    


    <!-- http://local.tamu.edu/djlee/ns/dqa#Disclaimer -->

    <owl:Class rdf:about="http://local.tamu.edu/djlee/ns/dqa#Disclaimer">
        <rdfs:subClassOf rdf:resource="http://www.w3.org/ns/dqv#QualityAnnotation"/>
        <rdfs:isDefinedBy>DDI</rdfs:isDefinedBy>
        <skos:definition>A disclaimer regarding the liability of the data producers or providers. Supports multiple language versions of the same content as well as optional formatting of the content.</skos:definition>
    </owl:Class>
    


    <!-- http://local.tamu.edu/djlee/ns/dqa#Dispute -->

    <owl:Class rdf:about="http://local.tamu.edu/djlee/ns/dqa#Dispute">
        <rdfs:subClassOf rdf:resource="http://www.w3.org/ns/dqv#QualityAnnotation"/>
        <rdfs:isDefinedBy>iso 9000</rdfs:isDefinedBy>
        <skos:definition>&lt;customer satisfaction&gt; disagreement, arising from a complaint (3.9.3), submitted to a DRP-provider</skos:definition>
    </owl:Class>
    


    <!-- http://local.tamu.edu/djlee/ns/dqa#DivisionOfLabor -->

    <owl:Class rdf:about="http://local.tamu.edu/djlee/ns/dqa#DivisionOfLabor">
        <rdfs:subClassOf rdf:resource="http://local.tamu.edu/djlee/ns/dqa#Tool"/>
        <rdfs:comment>Group (Organization and Community) mediates DQA Actvitity through Division Of Labor.
Division of Labor defines Activity specific allocation of Roles based on the Activity&apos;s set of Actions. 

Scenario  – Division of labor
In order to model the workflow and division of labor of the DQA process, John consults the ontology to identify the actions and roles involved in DQA. By utilizing the ontology, John is also able to determine who in the library’s organizational structure could be involved in the DQA process and their specific roles.</rdfs:comment>
    </owl:Class>
    


    <!-- http://local.tamu.edu/djlee/ns/dqa#EducationalProgram -->

    <owl:Class rdf:about="http://local.tamu.edu/djlee/ns/dqa#EducationalProgram">
        <rdfs:subClassOf rdf:resource="http://local.tamu.edu/djlee/ns/dqa#ProfessionalDevelopment"/>
        <rdfs:isDefinedBy>IQAF</rdfs:isDefinedBy>
    </owl:Class>
    


    <!-- http://local.tamu.edu/djlee/ns/dqa#InformationProduct -->

    <owl:Class rdf:about="http://local.tamu.edu/djlee/ns/dqa#InformationProduct">
        <owl:equivalentClass>
            <owl:Restriction>
                <owl:onProperty rdf:resource="http://local.tamu.edu/djlee/ns/dqa#hasQualityActiveModel"/>
                <owl:someValuesFrom rdf:resource="http://local.tamu.edu/djlee/ns/dqa#Quality_Model_Active"/>
            </owl:Restriction>
        </owl:equivalentClass>
        <owl:equivalentClass>
            <owl:Restriction>
                <owl:onProperty rdf:resource="http://local.tamu.edu/djlee/ns/dqa#hasQualityProblem"/>
                <owl:someValuesFrom rdf:resource="http://local.tamu.edu/djlee/ns/dqa#Quality_Problem"/>
            </owl:Restriction>
        </owl:equivalentClass>
        <owl:equivalentClass>
            <owl:Restriction>
                <owl:onProperty rdf:resource="http://local.tamu.edu/djlee/ns/dqa#hasQualityRequiredModel"/>
                <owl:someValuesFrom rdf:resource="http://local.tamu.edu/djlee/ns/dqa#Quality_Model_Required"/>
            </owl:Restriction>
        </owl:equivalentClass>
        <owl:equivalentClass>
            <owl:Restriction>
                <owl:onProperty rdf:resource="http://local.tamu.edu/djlee/ns/dqa#requiresExpertise"/>
                <owl:someValuesFrom rdf:resource="https://www.w3.org/TR/prov-o/#Agent"/>
            </owl:Restriction>
        </owl:equivalentClass>
        <owl:equivalentClass>
            <owl:Restriction>
                <owl:onProperty rdf:resource="http://www.w3.org/TR/prov-o#isAttributedTo"/>
                <owl:someValuesFrom rdf:resource="https://www.w3.org/TR/prov-o/#Activity"/>
            </owl:Restriction>
        </owl:equivalentClass>
        <owl:equivalentClass>
            <owl:Restriction>
                <owl:onProperty rdf:resource="http://www.w3.org/TR/prov-o#isAttributedTo"/>
                <owl:someValuesFrom rdf:resource="https://www.w3.org/TR/prov-o/#Agent"/>
            </owl:Restriction>
        </owl:equivalentClass>
        <owl:equivalentClass>
            <owl:Restriction>
                <owl:onProperty rdf:resource="http://www.w3.org/TR/prov-o#isDerivedFrom"/>
                <owl:someValuesFrom rdf:resource="https://www.w3.org/TR/prov-o/#Activity"/>
            </owl:Restriction>
        </owl:equivalentClass>
        <owl:equivalentClass>
            <owl:Restriction>
                <owl:onProperty rdf:resource="http://www.w3.org/TR/prov-o#isDerivedFrom"/>
                <owl:someValuesFrom rdf:resource="https://www.w3.org/TR/prov-o/#Agent"/>
            </owl:Restriction>
        </owl:equivalentClass>
        <owl:equivalentClass>
            <owl:Restriction>
                <owl:onProperty rdf:resource="http://www.w3.org/TR/prov-o#isGeneratedBy"/>
                <owl:someValuesFrom rdf:resource="https://www.w3.org/TR/prov-o/#Activity"/>
            </owl:Restriction>
        </owl:equivalentClass>
        <owl:equivalentClass>
            <owl:Restriction>
                <owl:onProperty rdf:resource="http://www.w3.org/TR/prov-o#isGeneratedBy"/>
                <owl:someValuesFrom rdf:resource="https://www.w3.org/TR/prov-o/#Agent"/>
            </owl:Restriction>
        </owl:equivalentClass>
        <owl:equivalentClass>
            <owl:Restriction>
                <owl:onProperty rdf:resource="https://www.w3.org/TR/vocab-duv/#hasDistributor"/>
                <owl:someValuesFrom rdf:resource="https://www.w3.org/TR/prov-o/#Agent"/>
            </owl:Restriction>
        </owl:equivalentClass>
        <rdfs:seeAlso>Main class for Information/Data Product.</rdfs:seeAlso>
    </owl:Class>
    


    <!-- http://local.tamu.edu/djlee/ns/dqa#Insert -->

    <owl:Class rdf:about="http://local.tamu.edu/djlee/ns/dqa#Insert">
        <owl:equivalentClass>
            <owl:Restriction>
                <owl:onProperty rdf:resource="http://www.semanticweb.org/djlee/ontologies/2023/8/untitled-ontology-71#targets"/>
                <owl:someValuesFrom rdf:resource="http://local.tamu.edu/djlee/ns/dqa#InformationProduct"/>
            </owl:Restriction>
        </owl:equivalentClass>
        <rdfs:subClassOf rdf:resource="http://www.semanticweb.org/djlee/ontologies/2023/8/untitled-ontology-71#Action"/>
        <skos:definition>The act of adding at a specific location in an ordered collection.
 (Schema.org)</skos:definition>
    </owl:Class>
    


    <!-- http://local.tamu.edu/djlee/ns/dqa#InspectionResult -->

    <owl:Class rdf:about="http://local.tamu.edu/djlee/ns/dqa#InspectionResult">
        <rdfs:subClassOf rdf:resource="http://local.tamu.edu/djlee/ns/dqa#DataQuality"/>
        <rdfs:subClassOf rdf:resource="http://local.tamu.edu/djlee/ns/dqa#MetadataQuality"/>
        <rdfs:isDefinedBy>iso 8000</rdfs:isDefinedBy>
        <skos:definition>&lt;quality of product shape data&gt; result of inspection (.3..12.,_6_) to determine whether or not product data (3.5.3) contain data quality defects (3.12 .5)</skos:definition>
    </owl:Class>
    


    <!-- http://local.tamu.edu/djlee/ns/dqa#Instrument -->

    <owl:Class rdf:about="http://local.tamu.edu/djlee/ns/dqa#Instrument">
        <rdfs:subClassOf rdf:resource="http://local.tamu.edu/djlee/ns/dqa#Tool"/>
        <rdfs:comment>How different is Instrument from Measuring Equipment</rdfs:comment>
    </owl:Class>
    


    <!-- http://local.tamu.edu/djlee/ns/dqa#Intervention -->

    <owl:Class rdf:about="http://local.tamu.edu/djlee/ns/dqa#Intervention">
        <owl:equivalentClass>
            <owl:Restriction>
                <owl:onProperty rdf:resource="http://www.semanticweb.org/djlee/ontologies/2023/8/untitled-ontology-71#composedOf"/>
                <owl:someValuesFrom rdf:resource="http://local.tamu.edu/djlee/ns/dqa#Add"/>
            </owl:Restriction>
        </owl:equivalentClass>
        <owl:equivalentClass>
            <owl:Restriction>
                <owl:onProperty rdf:resource="http://www.semanticweb.org/djlee/ontologies/2023/8/untitled-ontology-71#composedOf"/>
                <owl:someValuesFrom rdf:resource="http://local.tamu.edu/djlee/ns/dqa#Correction"/>
            </owl:Restriction>
        </owl:equivalentClass>
        <owl:equivalentClass>
            <owl:Restriction>
                <owl:onProperty rdf:resource="http://www.semanticweb.org/djlee/ontologies/2023/8/untitled-ontology-71#composedOf"/>
                <owl:someValuesFrom rdf:resource="http://local.tamu.edu/djlee/ns/dqa#CorrectiveAction"/>
            </owl:Restriction>
        </owl:equivalentClass>
        <owl:equivalentClass>
            <owl:Restriction>
                <owl:onProperty rdf:resource="http://www.semanticweb.org/djlee/ontologies/2023/8/untitled-ontology-71#composedOf"/>
                <owl:someValuesFrom rdf:resource="http://local.tamu.edu/djlee/ns/dqa#Delete"/>
            </owl:Restriction>
        </owl:equivalentClass>
        <owl:equivalentClass>
            <owl:Restriction>
                <owl:onProperty rdf:resource="http://www.semanticweb.org/djlee/ontologies/2023/8/untitled-ontology-71#composedOf"/>
                <owl:someValuesFrom rdf:resource="http://local.tamu.edu/djlee/ns/dqa#Insert"/>
            </owl:Restriction>
        </owl:equivalentClass>
        <owl:equivalentClass>
            <owl:Restriction>
                <owl:onProperty rdf:resource="http://www.semanticweb.org/djlee/ontologies/2023/8/untitled-ontology-71#composedOf"/>
                <owl:someValuesFrom rdf:resource="http://local.tamu.edu/djlee/ns/dqa#PreventiveAction"/>
            </owl:Restriction>
        </owl:equivalentClass>
        <owl:equivalentClass>
            <owl:Restriction>
                <owl:onProperty rdf:resource="http://www.semanticweb.org/djlee/ontologies/2023/8/untitled-ontology-71#composedOf"/>
                <owl:someValuesFrom rdf:resource="http://local.tamu.edu/djlee/ns/dqa#Repair"/>
            </owl:Restriction>
        </owl:equivalentClass>
        <owl:equivalentClass>
            <owl:Restriction>
                <owl:onProperty rdf:resource="http://www.semanticweb.org/djlee/ontologies/2023/8/untitled-ontology-71#composedOf"/>
                <owl:someValuesFrom rdf:resource="http://local.tamu.edu/djlee/ns/dqa#Replace"/>
            </owl:Restriction>
        </owl:equivalentClass>
        <owl:equivalentClass>
            <owl:Restriction>
                <owl:onProperty rdf:resource="http://www.semanticweb.org/djlee/ontologies/2023/8/untitled-ontology-71#composedOf"/>
                <owl:someValuesFrom rdf:resource="http://www.semanticweb.org/djlee/ontologies/2023/8/untitled-ontology-71#Revision"/>
            </owl:Restriction>
        </owl:equivalentClass>
        <owl:equivalentClass>
            <owl:Restriction>
                <owl:onProperty rdf:resource="http://www.semanticweb.org/djlee/ontologies/2023/8/untitled-ontology-71#composedOf"/>
                <owl:someValuesFrom rdf:resource="http://www.semanticweb.org/djlee/ontologies/2023/8/untitled-ontology-71#Rework"/>
            </owl:Restriction>
        </owl:equivalentClass>
        <owl:equivalentClass>
            <owl:Restriction>
                <owl:onProperty rdf:resource="http://www.semanticweb.org/djlee/ontologies/2023/8/untitled-ontology-71#composedOf"/>
                <owl:someValuesFrom rdf:resource="http://www.semanticweb.org/djlee/ontologies/2023/8/untitled-ontology-71#Scrap"/>
            </owl:Restriction>
        </owl:equivalentClass>
        <owl:equivalentClass>
            <owl:Restriction>
                <owl:onProperty rdf:resource="http://www.semanticweb.org/djlee/ontologies/2023/8/untitled-ontology-71#composedOf"/>
                <owl:someValuesFrom rdf:resource="http://www.semanticweb.org/djlee/ontologies/2023/8/untitled-ontology-71#Update"/>
            </owl:Restriction>
        </owl:equivalentClass>
        <owl:equivalentClass>
            <owl:Restriction>
                <owl:onProperty rdf:resource="http://www.w3.org/ns/oa#motivatedBy"/>
                <owl:someValuesFrom rdf:resource="http://local.tamu.edu/djlee/ns/dqa#Quality_Objective"/>
            </owl:Restriction>
        </owl:equivalentClass>
        <rdfs:subClassOf rdf:resource="https://www.w3.org/TR/prov-o/#Activity"/>
        <rdfs:comment>Intervention class describes an intervention activity in the quality of a data product. 
Intervention comprises intervention Actions. 
Agent can enhance data product quality by intervining and preventing data Quality Problems. 
Agent can enhance data product quality by intervining in the data product itself, by scrapping or reworking the product.</rdfs:comment>
    </owl:Class>
    


    <!-- http://local.tamu.edu/djlee/ns/dqa#IntrinsicDimension -->

    <owl:Class rdf:about="http://local.tamu.edu/djlee/ns/dqa#IntrinsicDimension">
        <rdfs:subClassOf rdf:resource="http://www.w3.org/ns/dqv#Dimension"/>
        <rdfs:comment>Intrinsic DQ can be assessed by measuring internal/intrinsic characteristics of data in relation to some general or context specific reference source (e.g., scientific reference databases and models,  standards or sources of a particular culture).</rdfs:comment>
    </owl:Class>
    


    <!-- http://local.tamu.edu/djlee/ns/dqa#Manager -->

    <owl:Class rdf:about="http://local.tamu.edu/djlee/ns/dqa#Manager">
        <rdfs:subClassOf rdf:resource="http://local.tamu.edu/djlee/ns/dqa#Curator"/>
        <skos:definition>DQA
Person or group of people who directs and controls DQA tasks at higher level

ISO9000
Person or group of people who directs and controls an organization at the highest level</skos:definition>
    </owl:Class>
    


    <!-- http://local.tamu.edu/djlee/ns/dqa#MeasuringEquipment -->

    <owl:Class rdf:about="http://local.tamu.edu/djlee/ns/dqa#MeasuringEquipment">
        <rdfs:subClassOf rdf:resource="http://local.tamu.edu/djlee/ns/dqa#Tool"/>
        <rdfs:isDefinedBy>ISO 9000</rdfs:isDefinedBy>
        <skos:definition>measuring instrument, software, measurement standard, reference material or auxiliary apparatus or combination thereof necessary to realize a measurement process</skos:definition>
    </owl:Class>
    


    <!-- http://local.tamu.edu/djlee/ns/dqa#Metadata -->

    <owl:Class rdf:about="http://local.tamu.edu/djlee/ns/dqa#Metadata">
        <rdfs:subClassOf rdf:resource="http://local.tamu.edu/djlee/ns/dqa#InformationProduct"/>
        <rdfs:comment>Describes the metadata part of the data product.</rdfs:comment>
    </owl:Class>
    


    <!-- http://local.tamu.edu/djlee/ns/dqa#MetadataQuality -->

    <owl:Class rdf:about="http://local.tamu.edu/djlee/ns/dqa#MetadataQuality">
        <rdfs:subClassOf rdf:resource="http://www.w3.org/ns/dqv#QualityAnnotation"/>
        <rdfs:isDefinedBy>DDI</rdfs:isDefinedBy>
        <skos:definition>An assessment of the quality of the metadata within the Maintainable object,</skos:definition>
    </owl:Class>
    


    <!-- http://local.tamu.edu/djlee/ns/dqa#Mission -->

    <owl:Class rdf:about="http://local.tamu.edu/djlee/ns/dqa#Mission">
        <rdfs:subClassOf rdf:resource="http://local.tamu.edu/djlee/ns/dqa#ReferenceSource"/>
        <rdfs:isDefinedBy>ISO 9000</rdfs:isDefinedBy>
        <skos:definition>organization&apos;s purpose for existing as expressed by top management</skos:definition>
    </owl:Class>
    


    <!-- http://local.tamu.edu/djlee/ns/dqa#PreventiveAction -->

    <owl:Class rdf:about="http://local.tamu.edu/djlee/ns/dqa#PreventiveAction">
        <owl:equivalentClass>
            <owl:Restriction>
                <owl:onProperty rdf:resource="http://www.semanticweb.org/djlee/ontologies/2023/8/untitled-ontology-71#targets"/>
                <owl:someValuesFrom rdf:resource="http://www.semanticweb.org/djlee/ontologies/2023/8/untitled-ontology-71#Creation"/>
            </owl:Restriction>
        </owl:equivalentClass>
        <rdfs:subClassOf rdf:resource="http://www.semanticweb.org/djlee/ontologies/2023/8/untitled-ontology-71#Action"/>
        <skos:definition>ISO9000:
Action to eliminate the cause of a potential nonconformithy or other potential undesirable situation</skos:definition>
    </owl:Class>
    


    <!-- http://local.tamu.edu/djlee/ns/dqa#ProcessMetadata -->

    <owl:Class rdf:about="http://local.tamu.edu/djlee/ns/dqa#ProcessMetadata">
        <rdfs:subClassOf rdf:resource="http://local.tamu.edu/djlee/ns/dqa#Metadata"/>
        <rdfs:isDefinedBy>Wikipedia</rdfs:isDefinedBy>
        <skos:definition>Process metadata is used to describe the results of various operations in the data warehouse.</skos:definition>
    </owl:Class>
    


    <!-- http://local.tamu.edu/djlee/ns/dqa#ProductDimension -->

    <owl:Class rdf:about="http://local.tamu.edu/djlee/ns/dqa#ProductDimension">
        <rdfs:subClassOf rdf:resource="http://www.w3.org/ns/dqv#Dimension"/>
        <rdfs:comment>. DQAO’s product-level category, on the other hand, combines the reputational dimension with platform and organizational characteristics and requirements for a data product that makes it usable.</rdfs:comment>
    </owl:Class>
    


    <!-- http://local.tamu.edu/djlee/ns/dqa#ProfessionalDevelopment -->

    <owl:Class rdf:about="http://local.tamu.edu/djlee/ns/dqa#ProfessionalDevelopment">
        <owl:equivalentClass>
            <owl:Restriction>
                <owl:onProperty rdf:resource="https://www.w3.org/TR/prov-o/#isAssociatedWith"/>
                <owl:someValuesFrom rdf:resource="http://www.semanticweb.org/djlee/ontologies/2023/8/untitled-ontology-71#Group"/>
            </owl:Restriction>
        </owl:equivalentClass>
        <rdfs:subClassOf rdf:resource="http://local.tamu.edu/djlee/ns/dqa#Tool"/>
        <rdfs:isDefinedBy>IQAF</rdfs:isDefinedBy>
    </owl:Class>
    


    <!-- http://local.tamu.edu/djlee/ns/dqa#ProvenanceMetadata -->

    <owl:Class rdf:about="http://local.tamu.edu/djlee/ns/dqa#ProvenanceMetadata">
        <rdfs:subClassOf rdf:resource="http://local.tamu.edu/djlee/ns/dqa#ProcessMetadata"/>
        <rdfs:comment>Provenance Metadata is a record of the Activities involved in the creation and manipulation of a Data Product.</rdfs:comment>
    </owl:Class>
    


    <!-- http://local.tamu.edu/djlee/ns/dqa#Provider -->

    <owl:Class rdf:about="http://local.tamu.edu/djlee/ns/dqa#Provider">
        <owl:equivalentClass>
            <owl:Restriction>
                <owl:onProperty rdf:resource="http://www.semanticweb.org/djlee/ontologies/2023/8/untitled-ontology-71#provides"/>
                <owl:someValuesFrom rdf:resource="http://local.tamu.edu/djlee/ns/dqa#InformationProduct"/>
            </owl:Restriction>
        </owl:equivalentClass>
        <rdfs:subClassOf rdf:resource="https://www.w3.org/TR/prov-o/#Person"/>
        <rdfs:seeAlso>ISO9000
Person or organizaiton that could or does receive a product or a service that is intended for or required by this person or organization</rdfs:seeAlso>
    </owl:Class>
    


    <!-- http://local.tamu.edu/djlee/ns/dqa#QualityModel -->

    <owl:Class rdf:about="http://local.tamu.edu/djlee/ns/dqa#QualityModel">
        <rdfs:subClassOf rdf:resource="http://local.tamu.edu/djlee/ns/dqa#Quality_Objective"/>
        <rdfs:comment>The set of attributes that are used to define a Quality Objective.

Scenario
John is a new data curator at University X&apos;s Research Data Repository (RDR). His task is to create a Data Quality Assurance (DQA) process that aligns with the NSTC guidelines for desirable characteristics of data repositories. To begin conceptualizing the DQA process, John consults the Ontology to obtain a general model of the concept of data quality as a set of dimensions.  This helps him draft an initial objective of the DQA process, which is to achieve high data quality. He then shares this objective with RDR stakeholders to initiate discussions on defining data quality within their specific context.</rdfs:comment>
    </owl:Class>
    


    <!-- http://local.tamu.edu/djlee/ns/dqa#QualityScheme -->

    <owl:Class rdf:about="http://local.tamu.edu/djlee/ns/dqa#QualityScheme">
        <rdfs:subClassOf rdf:resource="http://local.tamu.edu/djlee/ns/dqa#ReferenceSource"/>
        <rdfs:isDefinedBy>Data Documentation Initiative</rdfs:isDefinedBy>
        <skos:definition>This scheme contains a set of quality statements and quality standards referenced by the metadata at different points in the lifecycle. In addition to the name, label, and description of the scheme, the structure supports the inclusion of another QualityScheme by reference and a set of QualityStatement descriptions either in-line or by reference.</skos:definition>
    </owl:Class>
    


    <!-- http://local.tamu.edu/djlee/ns/dqa#QualityStatement -->

    <owl:Class rdf:about="http://local.tamu.edu/djlee/ns/dqa#QualityStatement">
        <rdfs:subClassOf rdf:resource="http://www.w3.org/ns/dqv#QualityAnnotation"/>
        <rdfs:isDefinedBy>DDI</rdfs:isDefinedBy>
        <skos:definition>A statement of quality which may be related to an external standard or contain a simple statement of internal quality goals or expectations. When relating to an external standard information on compliance may be added providing a reference to a ComplianceConcept, an ExternalComplianceCode, as well as a description. Optionally, a general statement of quality may be provided using OtherQualityStatement.</skos:definition>
    </owl:Class>
    


    <!-- http://local.tamu.edu/djlee/ns/dqa#Quality_Model_Active -->

    <owl:Class rdf:about="http://local.tamu.edu/djlee/ns/dqa#Quality_Model_Active">
        <owl:equivalentClass>
            <owl:Restriction>
                <owl:onProperty rdf:resource="http://local.tamu.edu/djlee/ns/dqa#verifies"/>
                <owl:someValuesFrom rdf:resource="http://local.tamu.edu/djlee/ns/dqa#Quality_Model_Required"/>
            </owl:Restriction>
        </owl:equivalentClass>
        <rdfs:subClassOf rdf:resource="http://local.tamu.edu/djlee/ns/dqa#QualityModel"/>
        <rdfs:comment>the set of criteria operationalized through specific metrics are that used to measure the quaity of a dataset</rdfs:comment>
    </owl:Class>
    


    <!-- http://local.tamu.edu/djlee/ns/dqa#Quality_Model_Required -->

    <owl:Class rdf:about="http://local.tamu.edu/djlee/ns/dqa#Quality_Model_Required">
        <rdfs:subClassOf rdf:resource="http://local.tamu.edu/djlee/ns/dqa#QualityModel"/>
        <rdfs:comment>Defines specific levels of quality for the quality criteria of the active model that must be met to ensure the quality of a dataset.</rdfs:comment>
    </owl:Class>
    


    <!-- http://local.tamu.edu/djlee/ns/dqa#Quality_Objective -->

    <owl:Class rdf:about="http://local.tamu.edu/djlee/ns/dqa#Quality_Objective">
        <rdfs:subClassOf rdf:resource="http://www.semanticweb.org/djlee/ontologies/2023/8/untitled-ontology-71#Objective"/>
        <rdfs:comment>Quality related object or objective the RDR needs to obtain (source: ISO 9000).</rdfs:comment>
    </owl:Class>
    


    <!-- http://local.tamu.edu/djlee/ns/dqa#Quality_Problem -->

    <owl:Class rdf:about="http://local.tamu.edu/djlee/ns/dqa#Quality_Problem">
        <owl:equivalentClass>
            <owl:Restriction>
                <owl:onProperty rdf:resource="http://local.tamu.edu/djlee/ns/dqa#hasSource"/>
                <owl:someValuesFrom rdf:resource="http://www.semanticweb.org/djlee/ontologies/2023/8/untitled-ontology-71#Problem_Source"/>
            </owl:Restriction>
        </owl:equivalentClass>
        <owl:equivalentClass>
            <owl:Restriction>
                <owl:onProperty rdf:resource="http://local.tamu.edu/djlee/ns/dqa#identifierdBy"/>
                <owl:someValuesFrom rdf:resource="http://local.tamu.edu/djlee/ns/dqa#Quality_Model_Active"/>
            </owl:Restriction>
        </owl:equivalentClass>
        <rdfs:comment>Identifies issues in Information Product&apos;s current quality relative to the required quality levels indicated in Quality Model Required..</rdfs:comment>
    </owl:Class>
    


    <!-- http://local.tamu.edu/djlee/ns/dqa#QuantitativeResult -->

    <owl:Class rdf:about="http://local.tamu.edu/djlee/ns/dqa#QuantitativeResult">
        <rdfs:subClassOf rdf:resource="http://local.tamu.edu/djlee/ns/dqa#DataQuality"/>
        <rdfs:subClassOf rdf:resource="http://local.tamu.edu/djlee/ns/dqa#MetadataQuality"/>
        <rdfs:isDefinedBy>iso 19157</rdfs:isDefinedBy>
        <skos:definition>An annotation that associates a resource (especially, a dataset or a distribution) to another resource (for example, a document) that certifies the resource&apos;s quality according to a set of quality assessment rules.</skos:definition>
    </owl:Class>
    


    <!-- http://local.tamu.edu/djlee/ns/dqa#ReferenceMetadata -->

    <owl:Class rdf:about="http://local.tamu.edu/djlee/ns/dqa#ReferenceMetadata">
        <rdfs:subClassOf rdf:resource="http://local.tamu.edu/djlee/ns/dqa#Metadata"/>
        <rdfs:isDefinedBy>Data Cube</rdfs:isDefinedBy>
        <skos:definition>This is metadata that describes the dataset as a whole, such as categorization of the dataset, its publisher, and a SPARQL endpoint where it can be accessed. External metadata is described in section 9.</skos:definition>
    </owl:Class>
    


    <!-- http://local.tamu.edu/djlee/ns/dqa#ReferenceSource -->

    <owl:Class rdf:about="http://local.tamu.edu/djlee/ns/dqa#ReferenceSource">
        <owl:equivalentClass>
            <owl:Restriction>
                <owl:onProperty rdf:resource="http://www.semanticweb.org/djlee/ontologies/2023/8/untitled-ontology-71#targets"/>
                <owl:someValuesFrom rdf:resource="http://local.tamu.edu/djlee/ns/dqa#InformationProduct"/>
            </owl:Restriction>
        </owl:equivalentClass>
        <rdfs:subClassOf rdf:resource="http://local.tamu.edu/djlee/ns/dqa#Tool"/>
        <rdfs:comment>IDQAO:QualityAssessmentProcedure
Superclass for different assessment procedures.</rdfs:comment>
        <rdfs:comment>ISO19157</rdfs:comment>
        <rdfs:isDefinedBy>Oxford English Dictionary</rdfs:isDefinedBy>
        <skos:definition>Reference work</skos:definition>
    </owl:Class>
    


    <!-- http://local.tamu.edu/djlee/ns/dqa#Repair -->

    <owl:Class rdf:about="http://local.tamu.edu/djlee/ns/dqa#Repair">
        <owl:equivalentClass>
            <owl:Restriction>
                <owl:onProperty rdf:resource="http://www.semanticweb.org/djlee/ontologies/2023/8/untitled-ontology-71#targets"/>
                <owl:someValuesFrom rdf:resource="http://local.tamu.edu/djlee/ns/dqa#InformationProduct"/>
            </owl:Restriction>
        </owl:equivalentClass>
        <rdfs:subClassOf rdf:resource="http://www.semanticweb.org/djlee/ontologies/2023/8/untitled-ontology-71#Action"/>
        <skos:definition>ISO9000
Action on a nonconforming product or service to make it acceptable for the intended use</skos:definition>
    </owl:Class>
    


    <!-- http://local.tamu.edu/djlee/ns/dqa#Replace -->

    <owl:Class rdf:about="http://local.tamu.edu/djlee/ns/dqa#Replace">
        <owl:equivalentClass>
            <owl:Restriction>
                <owl:onProperty rdf:resource="http://www.semanticweb.org/djlee/ontologies/2023/8/untitled-ontology-71#targets"/>
                <owl:someValuesFrom rdf:resource="http://local.tamu.edu/djlee/ns/dqa#InformationProduct"/>
            </owl:Restriction>
        </owl:equivalentClass>
        <rdfs:subClassOf rdf:resource="http://www.semanticweb.org/djlee/ontologies/2023/8/untitled-ontology-71#Action"/>
        <skos:definition>The act of editing a recipient by replacing an old object with a new object.
(Schema.org)</skos:definition>
    </owl:Class>
    


    <!-- http://local.tamu.edu/djlee/ns/dqa#Role -->

    <owl:Class rdf:about="http://local.tamu.edu/djlee/ns/dqa#Role">
        <owl:equivalentClass>
            <owl:Restriction>
                <owl:onProperty rdf:resource="https://www.w3.org/TR/prov-o/#allocatedBy"/>
                <owl:someValuesFrom rdf:resource="http://local.tamu.edu/djlee/ns/dqa#DivisionOfLabor"/>
            </owl:Restriction>
        </owl:equivalentClass>
        <rdfs:subClassOf rdf:resource="http://local.tamu.edu/djlee/ns/dqa#Tool"/>
        <skos:definition>PROV:Role
A role is the function of an entity or agent with respect to an activity, in the context of a usage, generation, invalidation, association, start, and end.</skos:definition>
    </owl:Class>
    


    <!-- http://local.tamu.edu/djlee/ns/dqa#Scope -->

    <owl:Class rdf:about="http://local.tamu.edu/djlee/ns/dqa#Scope">
        <rdfs:subClassOf rdf:resource="http://local.tamu.edu/djlee/ns/dqa#ReferenceSource"/>
        <rdfs:isDefinedBy>Oxford English Dictionary</rdfs:isDefinedBy>
        <skos:definition>Something aimed at or desired; something which one wishes to effect or attain; an end in view; an object, purpose, aim.</skos:definition>
    </owl:Class>
    


    <!-- http://local.tamu.edu/djlee/ns/dqa#Software -->

    <owl:Class rdf:about="http://local.tamu.edu/djlee/ns/dqa#Software">
        <rdfs:subClassOf rdf:resource="http://local.tamu.edu/djlee/ns/dqa#Tool"/>
        <rdfs:comment>ISO16363</rdfs:comment>
        <rdfs:isDefinedBy>Schema.org</rdfs:isDefinedBy>
        <skos:definition>A software application</skos:definition>
    </owl:Class>
    


    <!-- http://local.tamu.edu/djlee/ns/dqa#Standard -->

    <owl:Class rdf:about="http://local.tamu.edu/djlee/ns/dqa#Standard">
        <rdfs:subClassOf rdf:resource="http://local.tamu.edu/djlee/ns/dqa#ReferenceSource"/>
        <rdfs:comment>Source: dcTerms</rdfs:comment>
        <rdfs:isDefinedBy>DublinCore</rdfs:isDefinedBy>
        <skos:definition>A reference point against which other things can be evaluated or compared.</skos:definition>
    </owl:Class>
    


    <!-- http://local.tamu.edu/djlee/ns/dqa#Strategy -->

    <owl:Class rdf:about="http://local.tamu.edu/djlee/ns/dqa#Strategy">
        <rdfs:subClassOf rdf:resource="http://local.tamu.edu/djlee/ns/dqa#ReferenceSource"/>
        <rdfs:isDefinedBy>ISO 9000</rdfs:isDefinedBy>
        <skos:definition>Plan to achieve a long-term or overall objective</skos:definition>
    </owl:Class>
    


    <!-- http://local.tamu.edu/djlee/ns/dqa#StructuralMetadata -->

    <owl:Class rdf:about="http://local.tamu.edu/djlee/ns/dqa#StructuralMetadata">
        <rdfs:subClassOf rdf:resource="http://local.tamu.edu/djlee/ns/dqa#Metadata"/>
        <rdfs:isDefinedBy>Data Cube</rdfs:isDefinedBy>
        <skos:definition>Having located an observation, we need certain metadata in order to be able to interpret it. What is the unit of measurement? Is it a normal value or a series break? Is the value measured or estimated? These metadata are provided as attributes and can be attached to individual observations, or to higher levels.</skos:definition>
    </owl:Class>
    


    <!-- http://local.tamu.edu/djlee/ns/dqa#Tool -->

    <owl:Class rdf:about="http://local.tamu.edu/djlee/ns/dqa#Tool">
        <rdfs:comment>This class describes Tools, including cognitive tools such as Methods, Metrics, Dimensions, Division of Labor, etc.</rdfs:comment>
    </owl:Class>
    


    <!-- http://local.tamu.edu/djlee/ns/dqa#User -->

    <owl:Class rdf:about="http://local.tamu.edu/djlee/ns/dqa#User">
        <rdfs:subClassOf rdf:resource="https://www.w3.org/TR/prov-o/#Person"/>
        <rdfs:isDefinedBy>ISO/IEC 25019</rdfs:isDefinedBy>
        <skos:definition>individual or group that interacts with a system or benefits from a system during its utilization</skos:definition>
    </owl:Class>
    


    <!-- http://local.tamu.edu/djlee/ns/dqa#Vision -->

    <owl:Class rdf:about="http://local.tamu.edu/djlee/ns/dqa#Vision">
        <rdfs:subClassOf rdf:resource="http://local.tamu.edu/djlee/ns/dqa#ReferenceSource"/>
        <rdfs:isDefinedBy>ISO 9000</rdfs:isDefinedBy>
        <skos:definition>Aspiration of what an organizaiton would like to become as expressed by top management</skos:definition>
    </owl:Class>
    


    <!-- http://local.tamu.edu/djlee/ns/dqa#prob_Activity_Contradiction -->

    <owl:Class rdf:about="http://local.tamu.edu/djlee/ns/dqa#prob_Activity_Contradiction">
        <rdfs:subClassOf rdf:resource="http://www.semanticweb.org/djlee/ontologies/2023/8/untitled-ontology-71#Problem_Source"/>
        <rdfs:comment>Congradictions in and between activity components causing quality problems.</rdfs:comment>
    </owl:Class>
    


    <!-- http://local.tamu.edu/djlee/ns/dqa#prob_Activity_Contradiction_Resource -->

    <owl:Class rdf:about="http://local.tamu.edu/djlee/ns/dqa#prob_Activity_Contradiction_Resource">
        <rdfs:subClassOf rdf:resource="http://local.tamu.edu/djlee/ns/dqa#prob_Activity_Contradiction"/>
        <rdfs:comment>The DQA Resource Provision related problems, includes human resources, their expertise. Source: ISO 8000 2016</rdfs:comment>
    </owl:Class>
    


    <!-- http://local.tamu.edu/djlee/ns/dqa#prob_Activity_Contradiction_Tools -->

    <owl:Class rdf:about="http://local.tamu.edu/djlee/ns/dqa#prob_Activity_Contradiction_Tools">
        <rdfs:subClassOf rdf:resource="http://local.tamu.edu/djlee/ns/dqa#prob_Activity_Contradiction"/>
        <rdfs:comment>Data management tool - infrastructure related problems. Source: ISO 8000-2016</rdfs:comment>
    </owl:Class>
    


    <!-- http://purl.org/spar/datacite/AgentIdentifier -->

    <owl:Class rdf:about="http://purl.org/spar/datacite/AgentIdentifier">
        <rdfs:subClassOf rdf:resource="http://purl.org/spar/datacite/Identifier"/>
        <rdfs:isDefinedBy>DataCite</rdfs:isDefinedBy>
        <skos:definition>Identifier for agent</skos:definition>
    </owl:Class>
    


    <!-- http://purl.org/spar/datacite/Identifier -->

    <owl:Class rdf:about="http://purl.org/spar/datacite/Identifier">
        <rdfs:subClassOf rdf:resource="http://local.tamu.edu/djlee/ns/dqa#Tool"/>
        <rdfs:comment>ISO16363</rdfs:comment>
        <rdfs:isDefinedBy>DataCite Metadata Schema</rdfs:isDefinedBy>
        <skos:definition>The Identifier is a unique string that identifies a resource.</skos:definition>
    </owl:Class>
    


    <!-- http://purl.org/spar/datacite/ResourceIdentifier -->

    <owl:Class rdf:about="http://purl.org/spar/datacite/ResourceIdentifier">
        <rdfs:subClassOf rdf:resource="http://purl.org/spar/datacite/Identifier"/>
        <rdfs:isDefinedBy>DataCite</rdfs:isDefinedBy>
        <skos:definition>Identifier for resource (e.g., instruments)</skos:definition>
    </owl:Class>
    


    <!-- http://www.semanticweb.org/djlee/ontologies/2023/8/untitled-ontology-71#Action -->

    <owl:Class rdf:about="http://www.semanticweb.org/djlee/ontologies/2023/8/untitled-ontology-71#Action">
        <owl:equivalentClass>
            <owl:Restriction>
                <owl:onProperty rdf:resource="http://www.semanticweb.org/djlee/ontologies/2023/8/untitled-ontology-71#composedOf"/>
                <owl:someValuesFrom rdf:resource="http://www.semanticweb.org/djlee/ontologies/2023/8/untitled-ontology-71#Action"/>
            </owl:Restriction>
        </owl:equivalentClass>
        <rdfs:comment>DQA Activities are comprised of Actions</rdfs:comment>
    </owl:Class>
    


    <!-- http://www.semanticweb.org/djlee/ontologies/2023/8/untitled-ontology-71#Activity_Type -->

    <owl:Class rdf:about="http://www.semanticweb.org/djlee/ontologies/2023/8/untitled-ontology-71#Activity_Type">
        <skos:definition>Different type of data intervention activities. 
https://doi.org/10.1002/asi.20652</skos:definition>
    </owl:Class>
    


    <!-- http://www.semanticweb.org/djlee/ontologies/2023/8/untitled-ontology-71#Approve -->

    <owl:Class rdf:about="http://www.semanticweb.org/djlee/ontologies/2023/8/untitled-ontology-71#Approve">
        <rdfs:subClassOf rdf:resource="http://www.semanticweb.org/djlee/ontologies/2023/8/untitled-ontology-71#Action"/>
        <skos:definition>To confirm authoritatively (OED)</skos:definition>
    </owl:Class>
    


    <!-- http://www.semanticweb.org/djlee/ontologies/2023/8/untitled-ontology-71#Ask -->

    <owl:Class rdf:about="http://www.semanticweb.org/djlee/ontologies/2023/8/untitled-ontology-71#Ask">
        <rdfs:subClassOf rdf:resource="http://www.semanticweb.org/djlee/ontologies/2023/8/untitled-ontology-71#Action"/>
        <skos:definition>The act of posing a question / favor to someone.
(Schema.org)</skos:definition>
    </owl:Class>
    


    <!-- http://www.semanticweb.org/djlee/ontologies/2023/8/untitled-ontology-71#Ask_permission_to_intervene -->

    <owl:Class rdf:about="http://www.semanticweb.org/djlee/ontologies/2023/8/untitled-ontology-71#Ask_permission_to_intervene">
        <rdfs:subClassOf rdf:resource="http://www.semanticweb.org/djlee/ontologies/2023/8/untitled-ontology-71#Action"/>
        <rdfs:comment>ISO9000 Permission
Action of giving formal authority

Not clear how this action is related to DQA? Is this about communicating about Accessibility?</rdfs:comment>
    </owl:Class>
    


    <!-- http://www.semanticweb.org/djlee/ontologies/2023/8/untitled-ontology-71#Assign -->

    <owl:Class rdf:about="http://www.semanticweb.org/djlee/ontologies/2023/8/untitled-ontology-71#Assign">
        <rdfs:subClassOf rdf:resource="http://www.semanticweb.org/djlee/ontologies/2023/8/untitled-ontology-71#Action"/>
        <skos:definition>The act of allocating an action/event/task to some destination (someone or something).
(Schema.org)</skos:definition>
    </owl:Class>
    


    <!-- http://www.semanticweb.org/djlee/ontologies/2023/8/untitled-ontology-71#Comment -->

    <owl:Class rdf:about="http://www.semanticweb.org/djlee/ontologies/2023/8/untitled-ontology-71#Comment">
        <rdfs:subClassOf rdf:resource="http://www.semanticweb.org/djlee/ontologies/2023/8/untitled-ontology-71#Action"/>
        <skos:definition>The act of generating a comment about a subject.
(Schema.org)</skos:definition>
    </owl:Class>
    


    <!-- http://www.semanticweb.org/djlee/ontologies/2023/8/untitled-ontology-71#Confirm -->

    <owl:Class rdf:about="http://www.semanticweb.org/djlee/ontologies/2023/8/untitled-ontology-71#Confirm">
        <rdfs:subClassOf rdf:resource="http://www.semanticweb.org/djlee/ontologies/2023/8/untitled-ontology-71#Action"/>
        <skos:definition>The act of notifying someone that a future event/action is going to happen as expected.
(Schema.org)</skos:definition>
    </owl:Class>
    


    <!-- http://www.semanticweb.org/djlee/ontologies/2023/8/untitled-ontology-71#Creation -->

    <owl:Class rdf:about="http://www.semanticweb.org/djlee/ontologies/2023/8/untitled-ontology-71#Creation">
        <rdfs:subClassOf rdf:resource="https://www.w3.org/TR/prov-o/#Activity"/>
        <rdfs:comment>This is data Creation activity.</rdfs:comment>
    </owl:Class>
    


    <!-- http://www.semanticweb.org/djlee/ontologies/2023/8/untitled-ontology-71#DQA_Evaluation -->

    <owl:Class rdf:about="http://www.semanticweb.org/djlee/ontologies/2023/8/untitled-ontology-71#DQA_Evaluation">
        <owl:equivalentClass>
            <owl:Restriction>
                <owl:onProperty rdf:resource="http://www.w3.org/ns/oa#motivatedBy"/>
                <owl:someValuesFrom rdf:resource="http://local.tamu.edu/djlee/ns/dqa#Quality_Objective"/>
            </owl:Restriction>
        </owl:equivalentClass>
        <rdfs:subClassOf rdf:resource="https://www.w3.org/TR/prov-o/#Activity"/>
        <rdfs:comment>Activity used to assess the design and operationalization of the DQA Process itself.</rdfs:comment>
    </owl:Class>
    


    <!-- http://www.semanticweb.org/djlee/ontologies/2023/8/untitled-ontology-71#DQA_Intervention -->

    <owl:Class rdf:about="http://www.semanticweb.org/djlee/ontologies/2023/8/untitled-ontology-71#DQA_Intervention">
        <owl:equivalentClass>
            <owl:Restriction>
                <owl:onProperty rdf:resource="http://www.w3.org/ns/oa#motivatedBy"/>
                <owl:someValuesFrom rdf:resource="http://local.tamu.edu/djlee/ns/dqa#Quality_Objective"/>
            </owl:Restriction>
        </owl:equivalentClass>
        <rdfs:subClassOf rdf:resource="https://www.w3.org/TR/prov-o/#Activity"/>
        <rdfs:comment>Activity is used describe interventions in the DQA Process itself.</rdfs:comment>
    </owl:Class>
    


    <!-- http://www.semanticweb.org/djlee/ontologies/2023/8/untitled-ontology-71#DQA_Process -->

    <owl:Class rdf:about="http://www.semanticweb.org/djlee/ontologies/2023/8/untitled-ontology-71#DQA_Process">
        <owl:equivalentClass>
            <owl:Restriction>
                <owl:onProperty rdf:resource="http://www.semanticweb.org/djlee/ontologies/2023/8/untitled-ontology-71#involvesCommunication"/>
                <owl:someValuesFrom rdf:resource="http://local.tamu.edu/djlee/ns/dqa#Communication"/>
            </owl:Restriction>
        </owl:equivalentClass>
        <owl:equivalentClass>
            <owl:Restriction>
                <owl:onProperty rdf:resource="http://www.semanticweb.org/djlee/ontologies/2023/8/untitled-ontology-71#involvesEvaluation"/>
                <owl:someValuesFrom rdf:resource="http://www.semanticweb.org/djlee/ontologies/2023/8/untitled-ontology-71#Evaluation"/>
            </owl:Restriction>
        </owl:equivalentClass>
        <owl:equivalentClass>
            <owl:Restriction>
                <owl:onProperty rdf:resource="http://www.semanticweb.org/djlee/ontologies/2023/8/untitled-ontology-71#involvesIntervention"/>
                <owl:someValuesFrom rdf:resource="http://local.tamu.edu/djlee/ns/dqa#Intervention"/>
            </owl:Restriction>
        </owl:equivalentClass>
        <rdfs:subClassOf rdf:resource="http://www.semanticweb.org/djlee/ontologies/2023/8/untitled-ontology-71#Process"/>
        <rdfs:comment>Represents the overall data quality assurance process, encompassing all activities aimed at ensuring data quality.</rdfs:comment>
    </owl:Class>
    


    <!-- http://www.semanticweb.org/djlee/ontologies/2023/8/untitled-ontology-71#DQA_Process_Improvement -->

    <owl:Class rdf:about="http://www.semanticweb.org/djlee/ontologies/2023/8/untitled-ontology-71#DQA_Process_Improvement">
        <owl:equivalentClass>
            <owl:Restriction>
                <owl:onProperty rdf:resource="http://www.semanticweb.org/djlee/ontologies/2023/8/untitled-ontology-71#evaluateDQA"/>
                <owl:someValuesFrom rdf:resource="http://www.semanticweb.org/djlee/ontologies/2023/8/untitled-ontology-71#DQA_Evaluation"/>
            </owl:Restriction>
        </owl:equivalentClass>
        <owl:equivalentClass>
            <owl:Restriction>
                <owl:onProperty rdf:resource="http://www.semanticweb.org/djlee/ontologies/2023/8/untitled-ontology-71#intervenesInDQA"/>
                <owl:someValuesFrom rdf:resource="http://www.semanticweb.org/djlee/ontologies/2023/8/untitled-ontology-71#DQA_Intervention"/>
            </owl:Restriction>
        </owl:equivalentClass>
        <rdfs:subClassOf rdf:resource="http://www.semanticweb.org/djlee/ontologies/2023/8/untitled-ontology-71#Process"/>
        <rdfs:comment>This class describes the process of a DQA Process improvement itself.</rdfs:comment>
    </owl:Class>
    


    <!-- http://www.semanticweb.org/djlee/ontologies/2023/8/untitled-ontology-71#Decontextualizing -->

    <owl:Class rdf:about="http://www.semanticweb.org/djlee/ontologies/2023/8/untitled-ontology-71#Decontextualizing">
        <rdfs:subClassOf rdf:resource="http://www.semanticweb.org/djlee/ontologies/2023/8/untitled-ontology-71#Activity_Type"/>
        <rdfs:comment>Decontextualizing ― activities that use information outside its original context of creation
(for instance, an activity may remove data products from their original contexts and
aggregate them into a new collection to support specific information needs or tasks.) 
https://doi.org/10.1002/asi.20652</rdfs:comment>
    </owl:Class>
    


    <!-- http://www.semanticweb.org/djlee/ontologies/2023/8/untitled-ontology-71#Define -->

    <owl:Class rdf:about="http://www.semanticweb.org/djlee/ontologies/2023/8/untitled-ontology-71#Define">
        <rdfs:subClassOf rdf:resource="http://www.semanticweb.org/djlee/ontologies/2023/8/untitled-ontology-71#Action"/>
        <skos:definition>To determine the boundary or spatial extent of; to settle the limits of. (OED)</skos:definition>
    </owl:Class>
    


    <!-- http://www.semanticweb.org/djlee/ontologies/2023/8/untitled-ontology-71#Evaluation -->

    <owl:Class rdf:about="http://www.semanticweb.org/djlee/ontologies/2023/8/untitled-ontology-71#Evaluation">
        <owl:equivalentClass>
            <owl:Restriction>
                <owl:onProperty rdf:resource="http://www.semanticweb.org/djlee/ontologies/2023/8/untitled-ontology-71#composedOf"/>
                <owl:someValuesFrom rdf:resource="http://www.semanticweb.org/djlee/ontologies/2023/8/untitled-ontology-71#Approve"/>
            </owl:Restriction>
        </owl:equivalentClass>
        <owl:equivalentClass>
            <owl:Restriction>
                <owl:onProperty rdf:resource="http://www.semanticweb.org/djlee/ontologies/2023/8/untitled-ontology-71#composedOf"/>
                <owl:someValuesFrom rdf:resource="http://www.semanticweb.org/djlee/ontologies/2023/8/untitled-ontology-71#Assign"/>
            </owl:Restriction>
        </owl:equivalentClass>
        <owl:equivalentClass>
            <owl:Restriction>
                <owl:onProperty rdf:resource="http://www.semanticweb.org/djlee/ontologies/2023/8/untitled-ontology-71#composedOf"/>
                <owl:someValuesFrom rdf:resource="http://www.semanticweb.org/djlee/ontologies/2023/8/untitled-ontology-71#Define"/>
            </owl:Restriction>
        </owl:equivalentClass>
        <owl:equivalentClass>
            <owl:Restriction>
                <owl:onProperty rdf:resource="http://www.semanticweb.org/djlee/ontologies/2023/8/untitled-ontology-71#composedOf"/>
                <owl:someValuesFrom rdf:resource="http://www.semanticweb.org/djlee/ontologies/2023/8/untitled-ontology-71#Measure"/>
            </owl:Restriction>
        </owl:equivalentClass>
        <owl:equivalentClass>
            <owl:Restriction>
                <owl:onProperty rdf:resource="http://www.semanticweb.org/djlee/ontologies/2023/8/untitled-ontology-71#composedOf"/>
                <owl:someValuesFrom rdf:resource="http://www.semanticweb.org/djlee/ontologies/2023/8/untitled-ontology-71#Observe"/>
            </owl:Restriction>
        </owl:equivalentClass>
        <owl:equivalentClass>
            <owl:Restriction>
                <owl:onProperty rdf:resource="http://www.semanticweb.org/djlee/ontologies/2023/8/untitled-ontology-71#composedOf"/>
                <owl:someValuesFrom rdf:resource="http://www.semanticweb.org/djlee/ontologies/2023/8/untitled-ontology-71#Organize"/>
            </owl:Restriction>
        </owl:equivalentClass>
        <owl:equivalentClass>
            <owl:Restriction>
                <owl:onProperty rdf:resource="http://www.semanticweb.org/djlee/ontologies/2023/8/untitled-ontology-71#composedOf"/>
                <owl:someValuesFrom rdf:resource="http://www.semanticweb.org/djlee/ontologies/2023/8/untitled-ontology-71#Plan"/>
            </owl:Restriction>
        </owl:equivalentClass>
        <owl:equivalentClass>
            <owl:Restriction>
                <owl:onProperty rdf:resource="http://www.w3.org/ns/oa#motivatedBy"/>
                <owl:someValuesFrom rdf:resource="http://local.tamu.edu/djlee/ns/dqa#Quality_Objective"/>
            </owl:Restriction>
        </owl:equivalentClass>
        <rdfs:subClassOf rdf:resource="https://www.w3.org/TR/prov-o/#Activity"/>
        <rdfs:comment>Evaluation activity includes quality conceptualization and measurement. 
Evaluation is performed by some Agent. 
Its Objective is to evaluate an informaiton product&apos;s quality. 
Evaluation is comprised of Action. 
It is mediated by Tool.</rdfs:comment>
    </owl:Class>
    


    <!-- http://www.semanticweb.org/djlee/ontologies/2023/8/untitled-ontology-71#FullInspection -->

    <owl:Class rdf:about="http://www.semanticweb.org/djlee/ontologies/2023/8/untitled-ontology-71#FullInspection">
        <owl:equivalentClass>
            <owl:Restriction>
                <owl:onProperty rdf:resource="http://www.semanticweb.org/djlee/ontologies/2023/8/untitled-ontology-71#usedIn"/>
                <owl:someValuesFrom rdf:resource="http://www.semanticweb.org/djlee/ontologies/2023/8/untitled-ontology-71#Evaluation"/>
            </owl:Restriction>
        </owl:equivalentClass>
        <rdfs:subClassOf rdf:resource="http://www.semanticweb.org/djlee/ontologies/2023/8/untitled-ontology-71#Method"/>
        <rdfs:isDefinedBy>ISO 9000</rdfs:isDefinedBy>
        <skos:definition>determination of conformity to specified requirements</skos:definition>
    </owl:Class>
    


    <!-- http://www.semanticweb.org/djlee/ontologies/2023/8/untitled-ontology-71#Group -->

    <owl:Class rdf:about="http://www.semanticweb.org/djlee/ontologies/2023/8/untitled-ontology-71#Group">
        <owl:equivalentClass>
            <owl:Restriction>
                <owl:onProperty rdf:resource="http://www.semanticweb.org/djlee/ontologies/2023/8/untitled-ontology-71#mediates"/>
                <owl:someValuesFrom rdf:resource="http://local.tamu.edu/djlee/ns/dqa#DivisionOfLabor"/>
            </owl:Restriction>
        </owl:equivalentClass>
        <owl:equivalentClass>
            <owl:Restriction>
                <owl:onProperty rdf:resource="http://www.semanticweb.org/djlee/ontologies/2023/8/untitled-ontology-71#mediates"/>
                <owl:someValuesFrom rdf:resource="http://local.tamu.edu/djlee/ns/dqa#ReferenceSource"/>
            </owl:Restriction>
        </owl:equivalentClass>
        <rdfs:subClassOf rdf:resource="https://www.w3.org/TR/prov-o/#Agent"/>
        <rdfs:comment>Used to describe the Agent type Group.</rdfs:comment>
    </owl:Class>
    


    <!-- http://www.semanticweb.org/djlee/ontologies/2023/8/untitled-ontology-71#IndirectEvaluation -->

    <owl:Class rdf:about="http://www.semanticweb.org/djlee/ontologies/2023/8/untitled-ontology-71#IndirectEvaluation">
        <owl:equivalentClass>
            <owl:Restriction>
                <owl:onProperty rdf:resource="http://www.semanticweb.org/djlee/ontologies/2023/8/untitled-ontology-71#usedIn"/>
                <owl:someValuesFrom rdf:resource="http://www.semanticweb.org/djlee/ontologies/2023/8/untitled-ontology-71#Evaluation"/>
            </owl:Restriction>
        </owl:equivalentClass>
        <rdfs:subClassOf rdf:resource="http://www.semanticweb.org/djlee/ontologies/2023/8/untitled-ontology-71#Method"/>
        <rdfs:isDefinedBy>ISO 19157</rdfs:isDefinedBy>
        <skos:definition>Method of evaluating the quality of a dataset based on external konwledge</skos:definition>
    </owl:Class>
    


    <!-- http://www.semanticweb.org/djlee/ontologies/2023/8/untitled-ontology-71#Inform -->

    <owl:Class rdf:about="http://www.semanticweb.org/djlee/ontologies/2023/8/untitled-ontology-71#Inform">
        <rdfs:subClassOf rdf:resource="http://www.semanticweb.org/djlee/ontologies/2023/8/untitled-ontology-71#Action"/>
        <skos:definition>The act of notifying someone of information pertinent to them, with no expectation of a response.
(Schema.org)</skos:definition>
    </owl:Class>
    


    <!-- http://www.semanticweb.org/djlee/ontologies/2023/8/untitled-ontology-71#Interact -->

    <owl:Class rdf:about="http://www.semanticweb.org/djlee/ontologies/2023/8/untitled-ontology-71#Interact">
        <rdfs:subClassOf rdf:resource="http://www.semanticweb.org/djlee/ontologies/2023/8/untitled-ontology-71#Action"/>
        <skos:definition>The act of interacting with another person or organization.
(Schema.org)</skos:definition>
    </owl:Class>
    


    <!-- http://www.semanticweb.org/djlee/ontologies/2023/8/untitled-ontology-71#Measure -->

    <owl:Class rdf:about="http://www.semanticweb.org/djlee/ontologies/2023/8/untitled-ontology-71#Measure">
        <rdfs:subClassOf rdf:resource="http://www.semanticweb.org/djlee/ontologies/2023/8/untitled-ontology-71#Action"/>
        <skos:definition>Process to determine a value (iso 9000)</skos:definition>
    </owl:Class>
    


    <!-- http://www.semanticweb.org/djlee/ontologies/2023/8/untitled-ontology-71#Measurement -->

    <owl:Class rdf:about="http://www.semanticweb.org/djlee/ontologies/2023/8/untitled-ontology-71#Measurement">
        <rdfs:subClassOf rdf:resource="http://www.semanticweb.org/djlee/ontologies/2023/8/untitled-ontology-71#Observation"/>
        <rdfs:comment>This is research measurements, research data</rdfs:comment>
    </owl:Class>
    


    <!-- http://www.semanticweb.org/djlee/ontologies/2023/8/untitled-ontology-71#Method -->

    <owl:Class rdf:about="http://www.semanticweb.org/djlee/ontologies/2023/8/untitled-ontology-71#Method">
        <rdfs:subClassOf rdf:resource="http://local.tamu.edu/djlee/ns/dqa#Tool"/>
        <rdfs:isDefinedBy>ISO 19157</rdfs:isDefinedBy>
        <skos:definition>the procedure used to evaluate the measure</skos:definition>
    </owl:Class>
    


    <!-- http://www.semanticweb.org/djlee/ontologies/2023/8/untitled-ontology-71#Monitor -->

    <owl:Class rdf:about="http://www.semanticweb.org/djlee/ontologies/2023/8/untitled-ontology-71#Monitor">
        <owl:equivalentClass>
            <owl:Restriction>
                <owl:onProperty rdf:resource="http://www.semanticweb.org/djlee/ontologies/2023/8/untitled-ontology-71#usedIn"/>
                <owl:someValuesFrom rdf:resource="http://www.semanticweb.org/djlee/ontologies/2023/8/untitled-ontology-71#Evaluation"/>
            </owl:Restriction>
        </owl:equivalentClass>
        <rdfs:subClassOf rdf:resource="http://www.semanticweb.org/djlee/ontologies/2023/8/untitled-ontology-71#Method"/>
        <rdfs:isDefinedBy>ISO 9000</rdfs:isDefinedBy>
        <skos:definition>determining the status of a system, a process, a product, a service, or an activity</skos:definition>
    </owl:Class>
    


    <!-- http://www.semanticweb.org/djlee/ontologies/2023/8/untitled-ontology-71#Objective -->

    <owl:Class rdf:about="http://www.semanticweb.org/djlee/ontologies/2023/8/untitled-ontology-71#Objective">
        <rdfs:comment>RDR&apos;s object - The objective the RDR nees to achieve.</rdfs:comment>
    </owl:Class>
    


    <!-- http://www.semanticweb.org/djlee/ontologies/2023/8/untitled-ontology-71#Observation -->

    <owl:Class rdf:about="http://www.semanticweb.org/djlee/ontologies/2023/8/untitled-ontology-71#Observation">
        <rdfs:isDefinedBy>OED</rdfs:isDefinedBy>
        <skos:definition>A single observation in the cube, may have one or more associated measured values. (source: Data Cube Vocabulary)</skos:definition>
        <skos:definition>The action or an act of observing, watching, or noticing; the fact or condition of being watched or noticed; notice; perception.</skos:definition>
    </owl:Class>
    


    <!-- http://www.semanticweb.org/djlee/ontologies/2023/8/untitled-ontology-71#Observe -->

    <owl:Class rdf:about="http://www.semanticweb.org/djlee/ontologies/2023/8/untitled-ontology-71#Observe">
        <rdfs:subClassOf rdf:resource="http://www.semanticweb.org/djlee/ontologies/2023/8/untitled-ontology-71#Action"/>
        <skos:definition>To follow, practise, or keep to (a mode of existence or conduct, a habit); to maintain or uphold (a quality, state, or condition, now esp. a silence or neutrality).  (OED)</skos:definition>
    </owl:Class>
    


    <!-- http://www.semanticweb.org/djlee/ontologies/2023/8/untitled-ontology-71#Organize -->

    <owl:Class rdf:about="http://www.semanticweb.org/djlee/ontologies/2023/8/untitled-ontology-71#Organize">
        <rdfs:subClassOf rdf:resource="http://www.semanticweb.org/djlee/ontologies/2023/8/untitled-ontology-71#Action"/>
        <skos:definition>The act of manipulating/administering/supervising/controlling one or more objects.
(Schema.org)</skos:definition>
    </owl:Class>
    


    <!-- http://www.semanticweb.org/djlee/ontologies/2023/8/untitled-ontology-71#Plan -->

    <owl:Class rdf:about="http://www.semanticweb.org/djlee/ontologies/2023/8/untitled-ontology-71#Plan">
        <rdfs:subClassOf rdf:resource="http://www.semanticweb.org/djlee/ontologies/2023/8/untitled-ontology-71#Action"/>
        <skos:definition>A plan is an entity that represents a set of actions or steps intended by one or more agents to achieve some goals.

(PROV Ontology)</skos:definition>
    </owl:Class>
    


    <!-- http://www.semanticweb.org/djlee/ontologies/2023/8/untitled-ontology-71#Problem_Source -->

    <owl:Class rdf:about="http://www.semanticweb.org/djlee/ontologies/2023/8/untitled-ontology-71#Problem_Source">
        <rdfs:comment>Data quality problem source.
https://doi.org/10.1002/asi.20652 
Stvilia&apos;s Information Quality Assessment Framework.</rdfs:comment>
    </owl:Class>
    


    <!-- http://www.semanticweb.org/djlee/ontologies/2023/8/untitled-ontology-71#Process -->

    <owl:Class rdf:about="http://www.semanticweb.org/djlee/ontologies/2023/8/untitled-ontology-71#Process">
        <rdfs:comment>Parent class for DQA Process.</rdfs:comment>
    </owl:Class>
    


    <!-- http://www.semanticweb.org/djlee/ontologies/2023/8/untitled-ontology-71#Provenance_Dependent -->

    <owl:Class rdf:about="http://www.semanticweb.org/djlee/ontologies/2023/8/untitled-ontology-71#Provenance_Dependent">
        <rdfs:subClassOf rdf:resource="http://www.semanticweb.org/djlee/ontologies/2023/8/untitled-ontology-71#Activity_Type"/>
        <rdfs:comment>Provenance-Dependent activities will be affected by any quality deficiencies in the creation and mediation process metadata of the information product. 
https://doi.org/10.1002/asi.20652</rdfs:comment>
    </owl:Class>
    


    <!-- http://www.semanticweb.org/djlee/ontologies/2023/8/untitled-ontology-71#Quality_Measurement -->

    <owl:Class rdf:about="http://www.semanticweb.org/djlee/ontologies/2023/8/untitled-ontology-71#Quality_Measurement">
        <owl:equivalentClass>
            <owl:Restriction>
                <owl:onProperty rdf:resource="http://www.w3.org/ns/dqv#isMeasurementOf"/>
                <owl:someValuesFrom rdf:resource="http://www.w3.org/ns/dqv#Metric"/>
            </owl:Restriction>
        </owl:equivalentClass>
        <rdfs:subClassOf rdf:resource="http://www.semanticweb.org/djlee/ontologies/2023/8/untitled-ontology-71#Observation"/>
        <rdfs:comment>Represents the evaluation of a specific data (source: DQV);
Describes quality measurements.</rdfs:comment>
    </owl:Class>
    


    <!-- http://www.semanticweb.org/djlee/ontologies/2023/8/untitled-ontology-71#Rate -->

    <owl:Class rdf:about="http://www.semanticweb.org/djlee/ontologies/2023/8/untitled-ontology-71#Rate">
        <owl:equivalentClass>
            <owl:Restriction>
                <owl:onProperty rdf:resource="http://www.semanticweb.org/djlee/ontologies/2023/8/untitled-ontology-71#usedIn"/>
                <owl:someValuesFrom rdf:resource="http://www.semanticweb.org/djlee/ontologies/2023/8/untitled-ontology-71#Evaluation"/>
            </owl:Restriction>
        </owl:equivalentClass>
        <rdfs:subClassOf rdf:resource="http://www.semanticweb.org/djlee/ontologies/2023/8/untitled-ontology-71#Method"/>
        <rdfs:isDefinedBy>Oxford English Dictionary</rdfs:isDefinedBy>
        <skos:definition>To be assessed or valued for purposes of taxation</skos:definition>
    </owl:Class>
    


    <!-- http://www.semanticweb.org/djlee/ontologies/2023/8/untitled-ontology-71#Release -->

    <owl:Class rdf:about="http://www.semanticweb.org/djlee/ontologies/2023/8/untitled-ontology-71#Release">
        <rdfs:subClassOf rdf:resource="http://www.semanticweb.org/djlee/ontologies/2023/8/untitled-ontology-71#Action"/>
        <skos:definition>permission to proceed to the next stage of a process (3.4.1) or the next process (iso 9000)</skos:definition>
    </owl:Class>
    


    <!-- http://www.semanticweb.org/djlee/ontologies/2023/8/untitled-ontology-71#Representation_Dependent -->

    <owl:Class rdf:about="http://www.semanticweb.org/djlee/ontologies/2023/8/untitled-ontology-71#Representation_Dependent">
        <rdfs:subClassOf rdf:resource="http://www.semanticweb.org/djlee/ontologies/2023/8/untitled-ontology-71#Activity_Type"/>
        <rdfs:comment>Representation Dependent ― activities that depend on how well data represents another entity, phenomenon, or event. 
https://doi.org/10.1002/asi.2065</rdfs:comment>
    </owl:Class>
    


    <!-- http://www.semanticweb.org/djlee/ontologies/2023/8/untitled-ontology-71#Review -->

    <owl:Class rdf:about="http://www.semanticweb.org/djlee/ontologies/2023/8/untitled-ontology-71#Review">
        <owl:equivalentClass>
            <owl:Restriction>
                <owl:onProperty rdf:resource="http://www.semanticweb.org/djlee/ontologies/2023/8/untitled-ontology-71#usedIn"/>
                <owl:someValuesFrom rdf:resource="http://www.semanticweb.org/djlee/ontologies/2023/8/untitled-ontology-71#Evaluation"/>
            </owl:Restriction>
        </owl:equivalentClass>
        <rdfs:subClassOf rdf:resource="http://www.semanticweb.org/djlee/ontologies/2023/8/untitled-ontology-71#Method"/>
        <rdfs:isDefinedBy>ISO 9000</rdfs:isDefinedBy>
        <skos:definition>determination of the suitability, adequacy or effectiveness of an object to achieve established objectives</skos:definition>
    </owl:Class>
    


    <!-- http://www.semanticweb.org/djlee/ontologies/2023/8/untitled-ontology-71#Revision -->

    <owl:Class rdf:about="http://www.semanticweb.org/djlee/ontologies/2023/8/untitled-ontology-71#Revision">
        <owl:equivalentClass>
            <owl:Restriction>
                <owl:onProperty rdf:resource="http://www.semanticweb.org/djlee/ontologies/2023/8/untitled-ontology-71#targets"/>
                <owl:someValuesFrom rdf:resource="http://local.tamu.edu/djlee/ns/dqa#InformationProduct"/>
            </owl:Restriction>
        </owl:equivalentClass>
        <rdfs:subClassOf rdf:resource="http://www.semanticweb.org/djlee/ontologies/2023/8/untitled-ontology-71#Action"/>
        <skos:definition>A revision is a derivation for which the resulting entity is a revised version of some original. The implication here is that the resulting entity contains substantial content from the original. Revision is a particular case of derivation.

(Prov Ontology)</skos:definition>
    </owl:Class>
    


    <!-- http://www.semanticweb.org/djlee/ontologies/2023/8/untitled-ontology-71#Rework -->

    <owl:Class rdf:about="http://www.semanticweb.org/djlee/ontologies/2023/8/untitled-ontology-71#Rework">
        <owl:equivalentClass>
            <owl:Restriction>
                <owl:onProperty rdf:resource="http://www.semanticweb.org/djlee/ontologies/2023/8/untitled-ontology-71#targets"/>
                <owl:someValuesFrom rdf:resource="http://local.tamu.edu/djlee/ns/dqa#InformationProduct"/>
            </owl:Restriction>
        </owl:equivalentClass>
        <rdfs:subClassOf rdf:resource="http://www.semanticweb.org/djlee/ontologies/2023/8/untitled-ontology-71#Action"/>
        <skos:definition>action on a nonconforming (3.6.9) product (3.7.6) or service (3.7.7) to make it conform to the requirements (3.6.4).  (iso 9000)</skos:definition>
    </owl:Class>
    


    <!-- http://www.semanticweb.org/djlee/ontologies/2023/8/untitled-ontology-71#SampleBasedInspection -->

    <owl:Class rdf:about="http://www.semanticweb.org/djlee/ontologies/2023/8/untitled-ontology-71#SampleBasedInspection">
        <owl:equivalentClass>
            <owl:Restriction>
                <owl:onProperty rdf:resource="http://www.semanticweb.org/djlee/ontologies/2023/8/untitled-ontology-71#usedIn"/>
                <owl:someValuesFrom rdf:resource="http://www.semanticweb.org/djlee/ontologies/2023/8/untitled-ontology-71#Evaluation"/>
            </owl:Restriction>
        </owl:equivalentClass>
        <rdfs:subClassOf rdf:resource="http://www.semanticweb.org/djlee/ontologies/2023/8/untitled-ontology-71#Method"/>
        <rdfs:isDefinedBy>ISO 9000, 8000</rdfs:isDefinedBy>
        <skos:definition>determination of conformity to specified requirements based on sample</skos:definition>
    </owl:Class>
    


    <!-- http://www.semanticweb.org/djlee/ontologies/2023/8/untitled-ontology-71#Scrap -->

    <owl:Class rdf:about="http://www.semanticweb.org/djlee/ontologies/2023/8/untitled-ontology-71#Scrap">
        <owl:equivalentClass>
            <owl:Restriction>
                <owl:onProperty rdf:resource="http://www.semanticweb.org/djlee/ontologies/2023/8/untitled-ontology-71#targets"/>
                <owl:someValuesFrom rdf:resource="http://local.tamu.edu/djlee/ns/dqa#InformationProduct"/>
            </owl:Restriction>
        </owl:equivalentClass>
        <rdfs:subClassOf rdf:resource="http://www.semanticweb.org/djlee/ontologies/2023/8/untitled-ontology-71#Action"/>
        <skos:definition>action on a nonconforming (3.6.9) product (3.7.6) or service (3.7.7) to preclude its originally intended use (iso 9000)</skos:definition>
    </owl:Class>
    


    <!-- http://www.semanticweb.org/djlee/ontologies/2023/8/untitled-ontology-71#Share -->

    <owl:Class rdf:about="http://www.semanticweb.org/djlee/ontologies/2023/8/untitled-ontology-71#Share">
        <rdfs:subClassOf rdf:resource="http://www.semanticweb.org/djlee/ontologies/2023/8/untitled-ontology-71#Action"/>
        <skos:definition>The act of distributing content to people for their amusement or edification.
(Schema.org)</skos:definition>
    </owl:Class>
    


    <!-- http://www.semanticweb.org/djlee/ontologies/2023/8/untitled-ontology-71#Stability_Dependent -->

    <owl:Class rdf:about="http://www.semanticweb.org/djlee/ontologies/2023/8/untitled-ontology-71#Stability_Dependent">
        <rdfs:subClassOf rdf:resource="http://www.semanticweb.org/djlee/ontologies/2023/8/untitled-ontology-71#Activity_Type"/>
        <rdfs:comment>Stability Dependent ― activities that depend on how stable the data product or its underlying entity(s) is
https://doi.org/10.1002/asi.2065</rdfs:comment>
    </owl:Class>
    


    <!-- http://www.semanticweb.org/djlee/ontologies/2023/8/untitled-ontology-71#Test -->

    <owl:Class rdf:about="http://www.semanticweb.org/djlee/ontologies/2023/8/untitled-ontology-71#Test">
        <owl:equivalentClass>
            <owl:Restriction>
                <owl:onProperty rdf:resource="http://www.semanticweb.org/djlee/ontologies/2023/8/untitled-ontology-71#usedIn"/>
                <owl:someValuesFrom rdf:resource="http://www.semanticweb.org/djlee/ontologies/2023/8/untitled-ontology-71#Evaluation"/>
            </owl:Restriction>
        </owl:equivalentClass>
        <rdfs:subClassOf rdf:resource="http://www.semanticweb.org/djlee/ontologies/2023/8/untitled-ontology-71#Method"/>
        <rdfs:isDefinedBy>ISO 9000</rdfs:isDefinedBy>
        <skos:definition>determination according to requirements for a specific intended use or application</skos:definition>
    </owl:Class>
    


    <!-- http://www.semanticweb.org/djlee/ontologies/2023/8/untitled-ontology-71#Update -->

    <owl:Class rdf:about="http://www.semanticweb.org/djlee/ontologies/2023/8/untitled-ontology-71#Update">
        <owl:equivalentClass>
            <owl:Restriction>
                <owl:onProperty rdf:resource="http://www.semanticweb.org/djlee/ontologies/2023/8/untitled-ontology-71#targets"/>
                <owl:someValuesFrom rdf:resource="http://local.tamu.edu/djlee/ns/dqa#InformationProduct"/>
            </owl:Restriction>
        </owl:equivalentClass>
        <rdfs:subClassOf rdf:resource="http://www.semanticweb.org/djlee/ontologies/2023/8/untitled-ontology-71#Action"/>
        <skos:definition>The act of managing by changing/editing the state of the object.
(Schema.org)</skos:definition>
    </owl:Class>
    


    <!-- http://www.semanticweb.org/djlee/ontologies/2023/8/untitled-ontology-71#prob_Changes_In_Data_Entity -->

    <owl:Class rdf:about="http://www.semanticweb.org/djlee/ontologies/2023/8/untitled-ontology-71#prob_Changes_In_Data_Entity">
        <owl:equivalentClass>
            <owl:Restriction>
                <owl:onProperty rdf:resource="http://www.semanticweb.org/djlee/ontologies/2023/8/untitled-ontology-71#affectsActivities"/>
                <owl:someValuesFrom rdf:resource="http://www.semanticweb.org/djlee/ontologies/2023/8/untitled-ontology-71#Provenance_Dependent"/>
            </owl:Restriction>
        </owl:equivalentClass>
        <owl:equivalentClass>
            <owl:Restriction>
                <owl:onProperty rdf:resource="http://www.semanticweb.org/djlee/ontologies/2023/8/untitled-ontology-71#affectsActivities"/>
                <owl:someValuesFrom rdf:resource="http://www.semanticweb.org/djlee/ontologies/2023/8/untitled-ontology-71#Stability_Dependent"/>
            </owl:Restriction>
        </owl:equivalentClass>
        <owl:equivalentClass>
            <owl:Restriction>
                <owl:onProperty rdf:resource="http://www.semanticweb.org/djlee/ontologies/2023/8/untitled-ontology-71#affectsDimensions"/>
                <owl:someValuesFrom rdf:resource="http://local.tamu.edu/djlee/ns/dqa#IntrinsicDimension"/>
            </owl:Restriction>
        </owl:equivalentClass>
        <owl:equivalentClass>
            <owl:Restriction>
                <owl:onProperty rdf:resource="http://www.semanticweb.org/djlee/ontologies/2023/8/untitled-ontology-71#affectsDimensions"/>
                <owl:someValuesFrom rdf:resource="http://local.tamu.edu/djlee/ns/dqa#ProductDimension"/>
            </owl:Restriction>
        </owl:equivalentClass>
        <rdfs:subClassOf rdf:resource="http://www.semanticweb.org/djlee/ontologies/2023/8/untitled-ontology-71#Problem_Source"/>
        <rdfs:comment>This class describes DQ problems caused by changes in the data itself.
https://doi.org/10.1002/asi.20652 Stvilia&apos;s Information Quality Assessment Framework.</rdfs:comment>
    </owl:Class>
    


    <!-- http://www.semanticweb.org/djlee/ontologies/2023/8/untitled-ontology-71#prob_Changes_In_Underlying_Entity -->

    <owl:Class rdf:about="http://www.semanticweb.org/djlee/ontologies/2023/8/untitled-ontology-71#prob_Changes_In_Underlying_Entity">
        <owl:equivalentClass>
            <owl:Restriction>
                <owl:onProperty rdf:resource="http://www.semanticweb.org/djlee/ontologies/2023/8/untitled-ontology-71#affectsActivities"/>
                <owl:someValuesFrom rdf:resource="http://www.semanticweb.org/djlee/ontologies/2023/8/untitled-ontology-71#Provenance_Dependent"/>
            </owl:Restriction>
        </owl:equivalentClass>
        <owl:equivalentClass>
            <owl:Restriction>
                <owl:onProperty rdf:resource="http://www.semanticweb.org/djlee/ontologies/2023/8/untitled-ontology-71#affectsActivities"/>
                <owl:someValuesFrom rdf:resource="http://www.semanticweb.org/djlee/ontologies/2023/8/untitled-ontology-71#Stability_Dependent"/>
            </owl:Restriction>
        </owl:equivalentClass>
        <owl:equivalentClass>
            <owl:Restriction>
                <owl:onProperty rdf:resource="http://www.semanticweb.org/djlee/ontologies/2023/8/untitled-ontology-71#affectsDimensions"/>
                <owl:someValuesFrom rdf:resource="http://local.tamu.edu/djlee/ns/dqa#ProductDimension"/>
            </owl:Restriction>
        </owl:equivalentClass>
        <rdfs:subClassOf rdf:resource="http://www.semanticweb.org/djlee/ontologies/2023/8/untitled-ontology-71#Problem_Source"/>
        <rdfs:comment>This class represents a type of DQ problems that occur in a data product due to changes in its underlying entity(s).</rdfs:comment>
    </owl:Class>
    


    <!-- http://www.semanticweb.org/djlee/ontologies/2023/8/untitled-ontology-71#prob_Context_Change -->

    <owl:Class rdf:about="http://www.semanticweb.org/djlee/ontologies/2023/8/untitled-ontology-71#prob_Context_Change">
        <owl:equivalentClass>
            <owl:Restriction>
                <owl:onProperty rdf:resource="http://www.semanticweb.org/djlee/ontologies/2023/8/untitled-ontology-71#affectsActivities"/>
                <owl:someValuesFrom rdf:resource="http://www.semanticweb.org/djlee/ontologies/2023/8/untitled-ontology-71#Decontextualizing"/>
            </owl:Restriction>
        </owl:equivalentClass>
        <owl:equivalentClass>
            <owl:Restriction>
                <owl:onProperty rdf:resource="http://www.semanticweb.org/djlee/ontologies/2023/8/untitled-ontology-71#affectsActivities"/>
                <owl:someValuesFrom rdf:resource="http://www.semanticweb.org/djlee/ontologies/2023/8/untitled-ontology-71#Provenance_Dependent"/>
            </owl:Restriction>
        </owl:equivalentClass>
        <owl:equivalentClass>
            <owl:Restriction>
                <owl:onProperty rdf:resource="http://www.semanticweb.org/djlee/ontologies/2023/8/untitled-ontology-71#affectsDimensions"/>
                <owl:someValuesFrom rdf:resource="http://local.tamu.edu/djlee/ns/dqa#ProductDimension"/>
            </owl:Restriction>
        </owl:equivalentClass>
        <rdfs:subClassOf rdf:resource="http://www.semanticweb.org/djlee/ontologies/2023/8/untitled-ontology-71#Problem_Source"/>
        <rdfs:comment>Any change in context, whether it be temporal or spatial, can change how DQ is
understood and evaluated, and can lead to an DQ problem. An data product can be of good quality in its original context but can become of lower quality once it is moved to a different context.
https://doi.org/10.1002/asi.20652</rdfs:comment>
    </owl:Class>
    


    <!-- http://www.semanticweb.org/djlee/ontologies/2023/8/untitled-ontology-71#prob_Mapping -->

    <owl:Class rdf:about="http://www.semanticweb.org/djlee/ontologies/2023/8/untitled-ontology-71#prob_Mapping">
        <owl:equivalentClass>
            <owl:Restriction>
                <owl:onProperty rdf:resource="http://www.semanticweb.org/djlee/ontologies/2023/8/untitled-ontology-71#affectsActivities"/>
                <owl:someValuesFrom rdf:resource="http://www.semanticweb.org/djlee/ontologies/2023/8/untitled-ontology-71#Provenance_Dependent"/>
            </owl:Restriction>
        </owl:equivalentClass>
        <owl:equivalentClass>
            <owl:Restriction>
                <owl:onProperty rdf:resource="http://www.semanticweb.org/djlee/ontologies/2023/8/untitled-ontology-71#affectsActivities"/>
                <owl:someValuesFrom rdf:resource="http://www.semanticweb.org/djlee/ontologies/2023/8/untitled-ontology-71#Representation_Dependent"/>
            </owl:Restriction>
        </owl:equivalentClass>
        <owl:equivalentClass>
            <owl:Restriction>
                <owl:onProperty rdf:resource="http://www.semanticweb.org/djlee/ontologies/2023/8/untitled-ontology-71#affectsDimensions"/>
                <owl:someValuesFrom rdf:resource="http://local.tamu.edu/djlee/ns/dqa#IntrinsicDimension"/>
            </owl:Restriction>
        </owl:equivalentClass>
        <owl:equivalentClass>
            <owl:Restriction>
                <owl:onProperty rdf:resource="http://www.semanticweb.org/djlee/ontologies/2023/8/untitled-ontology-71#affectsDimensions"/>
                <owl:someValuesFrom rdf:resource="http://local.tamu.edu/djlee/ns/dqa#ProductDimension"/>
            </owl:Restriction>
        </owl:equivalentClass>
        <rdfs:subClassOf rdf:resource="http://www.semanticweb.org/djlee/ontologies/2023/8/untitled-ontology-71#Problem_Source"/>
        <rdfs:comment>Mapping-related data quality problems arise when there is incomplete, ambiguous, inaccurate, inconsistent, or redundant mapping between some state, phenomenon, event, or entity and data.
https://doi.org/10.1002/asi.20652</rdfs:comment>
    </owl:Class>
    


    <!-- http://www.w3.org/ns/dqv#Dimension -->

    <owl:Class rdf:about="http://www.w3.org/ns/dqv#Dimension">
        <owl:equivalentClass>
            <owl:Restriction>
                <owl:onProperty rdf:resource="http://local.tamu.edu/djlee/ns/dqa#isPartOf"/>
                <owl:someValuesFrom rdf:resource="http://local.tamu.edu/djlee/ns/dqa#QualityModel"/>
            </owl:Restriction>
        </owl:equivalentClass>
        <owl:equivalentClass>
            <owl:Restriction>
                <owl:onProperty rdf:resource="http://www.semanticweb.org/djlee/ontologies/2023/8/untitled-ontology-71#isMeasuredBy"/>
                <owl:someValuesFrom rdf:resource="http://www.w3.org/ns/dqv#Metric"/>
            </owl:Restriction>
        </owl:equivalentClass>
        <rdfs:subClassOf rdf:resource="http://local.tamu.edu/djlee/ns/dqa#Tool"/>
        <rdfs:comment>DDI; Dcube; DUV:Motivation; OA:Motivation</rdfs:comment>
        <rdfs:isDefinedBy>OED</rdfs:isDefinedBy>
        <rdfs:seeAlso>DDI:QualityScheme</rdfs:seeAlso>
        <skos:definition>Measurable or spatial extent of any kind, as length, breadth, thickness, area, volume; measurement, measure, magnitude, size.</skos:definition>
    </owl:Class>
    


    <!-- http://www.w3.org/ns/dqv#Metric -->

    <owl:Class rdf:about="http://www.w3.org/ns/dqv#Metric">
        <owl:equivalentClass>
            <owl:Restriction>
                <owl:onProperty rdf:resource="https://www.w3.org/TR/vocab-duv/#refersTo"/>
                <owl:someValuesFrom rdf:resource="http://local.tamu.edu/djlee/ns/dqa#ReferenceSource"/>
            </owl:Restriction>
        </owl:equivalentClass>
        <rdfs:subClassOf rdf:resource="http://local.tamu.edu/djlee/ns/dqa#Tool"/>
        <rdfs:comment>This class is used to describe Metrics that operationalize Dimensions for use in data Evaluation Activities.</rdfs:comment>
    </owl:Class>
    


    <!-- http://www.w3.org/ns/dqv#QualityAnnotation -->

    <owl:Class rdf:about="http://www.w3.org/ns/dqv#QualityAnnotation">
        <owl:equivalentClass>
            <owl:Restriction>
                <owl:onProperty rdf:resource="http://www.semanticweb.org/djlee/ontologies/2023/8/untitled-ontology-71#comprisedOf"/>
                <owl:someValuesFrom rdf:resource="http://www.semanticweb.org/djlee/ontologies/2023/8/untitled-ontology-71#Quality_Measurement"/>
            </owl:Restriction>
        </owl:equivalentClass>
        <rdfs:subClassOf rdf:resource="http://local.tamu.edu/djlee/ns/dqa#Metadata"/>
        <rdfs:isDefinedBy>DQV</rdfs:isDefinedBy>
        <skos:definition>Represents quality annotations, including ratings, quality certificates or feedback that can be associated to datasets or distributions. Quality annotations must have one oa:motivatedBy statement with an instance of oa:Motivation (and skos:Concept) that reflects a quality assessment purpose. We define this instance as dqv:qualityAssessment.</skos:definition>
    </owl:Class>
    


    <!-- http://www.w3.org/ns/dqv#QualityCertificate -->

    <owl:Class rdf:about="http://www.w3.org/ns/dqv#QualityCertificate">
        <rdfs:subClassOf rdf:resource="http://www.w3.org/ns/dqv#QualityAnnotation"/>
        <rdfs:isDefinedBy>DQV</rdfs:isDefinedBy>
        <skos:definition>An annotation that associates a resource (especially, a dataset or a distribution) to another resource (for example, a document) that certifies the resource&apos;s quality according to a set of quality assessment rules.</skos:definition>
    </owl:Class>
    


    <!-- http://www.w3.org/ns/dqv#QualityPolicy -->

    <owl:Class rdf:about="http://www.w3.org/ns/dqv#QualityPolicy">
        <rdfs:subClassOf rdf:resource="http://local.tamu.edu/djlee/ns/dqa#ReferenceSource"/>
        <rdfs:isDefinedBy>ISO 9000</rdfs:isDefinedBy>
        <skos:definition>policy related to quality</skos:definition>
    </owl:Class>
    


    <!-- http://www.w3.org/ns/dqv#UserQualityFeedback -->

    <owl:Class rdf:about="http://www.w3.org/ns/dqv#UserQualityFeedback">
        <rdfs:subClassOf rdf:resource="http://www.w3.org/ns/dqv#QualityAnnotation"/>
        <rdfs:isDefinedBy>ISO 9000</rdfs:isDefinedBy>
        <skos:definition>&lt;customer satisfaction&gt; opinions, comments and expressions of interest in a product (3.7.6), a service (3.7.7) or a complaints-handling process (3.4.1)</skos:definition>
    </owl:Class>
    


    <!-- https://www.w3.org/TR/prov-o/#Activity -->

    <owl:Class rdf:about="https://www.w3.org/TR/prov-o/#Activity">
        <owl:equivalentClass>
            <owl:Restriction>
                <owl:onProperty rdf:resource="http://www.semanticweb.org/djlee/ontologies/2023/8/untitled-ontology-71#isMediatedBy"/>
                <owl:someValuesFrom rdf:resource="http://local.tamu.edu/djlee/ns/dqa#Tool"/>
            </owl:Restriction>
        </owl:equivalentClass>
        <owl:equivalentClass>
            <owl:Restriction>
                <owl:onProperty rdf:resource="http://www.semanticweb.org/djlee/ontologies/2023/8/untitled-ontology-71#isMediatedBy"/>
                <owl:someValuesFrom rdf:resource="http://www.semanticweb.org/djlee/ontologies/2023/8/untitled-ontology-71#Group"/>
            </owl:Restriction>
        </owl:equivalentClass>
        <owl:equivalentClass>
            <owl:Restriction>
                <owl:onProperty rdf:resource="http://www.semanticweb.org/djlee/ontologies/2023/8/untitled-ontology-71#isPerformedBy"/>
                <owl:someValuesFrom rdf:resource="https://www.w3.org/TR/prov-o/#Agent"/>
            </owl:Restriction>
        </owl:equivalentClass>
        <owl:equivalentClass>
            <owl:Restriction>
                <owl:onProperty rdf:resource="http://www.w3.org/ns/oa#motivatedBy"/>
                <owl:someValuesFrom rdf:resource="http://www.semanticweb.org/djlee/ontologies/2023/8/untitled-ontology-71#Objective"/>
            </owl:Restriction>
        </owl:equivalentClass>
        <rdfs:comment>PROV:Activity
An activity is something that occurs over a period of time and acts upon or with entities; it may include consuming, processing, transforming, modifying, relocating, using, or generating entities.</rdfs:comment>
    </owl:Class>
    


    <!-- https://www.w3.org/TR/prov-o/#Agent -->

    <owl:Class rdf:about="https://www.w3.org/TR/prov-o/#Agent">
        <owl:equivalentClass>
            <owl:Restriction>
                <owl:onProperty rdf:resource="http://local.tamu.edu/djlee/ns/dqa#collects"/>
                <owl:someValuesFrom rdf:resource="http://local.tamu.edu/djlee/ns/dqa#InformationProduct"/>
            </owl:Restriction>
        </owl:equivalentClass>
        <owl:equivalentClass>
            <owl:Restriction>
                <owl:onProperty rdf:resource="http://local.tamu.edu/djlee/ns/dqa#contributes"/>
                <owl:someValuesFrom rdf:resource="http://local.tamu.edu/djlee/ns/dqa#InformationProduct"/>
            </owl:Restriction>
        </owl:equivalentClass>
        <owl:equivalentClass>
            <owl:Restriction>
                <owl:onProperty rdf:resource="http://local.tamu.edu/djlee/ns/dqa#creates"/>
                <owl:someValuesFrom rdf:resource="http://local.tamu.edu/djlee/ns/dqa#InformationProduct"/>
            </owl:Restriction>
        </owl:equivalentClass>
        <owl:equivalentClass>
            <owl:Restriction>
                <owl:onProperty rdf:resource="http://www.semanticweb.org/djlee/ontologies/2023/8/untitled-ontology-71#mediates"/>
                <owl:someValuesFrom rdf:resource="http://local.tamu.edu/djlee/ns/dqa#Tool"/>
            </owl:Restriction>
        </owl:equivalentClass>
        <owl:equivalentClass>
            <owl:Restriction>
                <owl:onProperty rdf:resource="http://www.semanticweb.org/djlee/ontologies/2023/8/untitled-ontology-71#playRole"/>
                <owl:someValuesFrom rdf:resource="http://local.tamu.edu/djlee/ns/dqa#Role"/>
            </owl:Restriction>
        </owl:equivalentClass>
        <owl:equivalentClass>
            <owl:Restriction>
                <owl:onProperty rdf:resource="https://www.w3.org/TR/prov-o/#hasPrimarySource"/>
                <owl:someValuesFrom rdf:resource="http://local.tamu.edu/djlee/ns/dqa#Metadata"/>
            </owl:Restriction>
        </owl:equivalentClass>
        <owl:equivalentClass>
            <owl:Restriction>
                <owl:onProperty rdf:resource="https://www.w3.org/TR/prov-o/#hasPrimarySource"/>
                <owl:someValuesFrom rdf:resource="http://local.tamu.edu/djlee/ns/dqa#ReferenceSource"/>
            </owl:Restriction>
        </owl:equivalentClass>
        <owl:equivalentClass>
            <owl:Restriction>
                <owl:onProperty rdf:resource="https://www.w3.org/TR/prov-o/#used"/>
                <owl:someValuesFrom rdf:resource="http://local.tamu.edu/djlee/ns/dqa#InformationProduct"/>
            </owl:Restriction>
        </owl:equivalentClass>
        <owl:equivalentClass>
            <owl:Restriction>
                <owl:onProperty rdf:resource="https://www.w3.org/TR/vocab-duv/#hasFeedback"/>
                <owl:someValuesFrom rdf:resource="http://www.w3.org/ns/dqv#UserQualityFeedback"/>
            </owl:Restriction>
        </owl:equivalentClass>
        <rdfs:seeAlso>DDI: AgentType</rdfs:seeAlso>
        <rdfs:seeAlso>PROV:Agent
An agent is something that bears some form of responsibility for an activity taking place, for the existence of an entity, or for another agent&apos;s activity.</rdfs:seeAlso>
    </owl:Class>
    


    <!-- https://www.w3.org/TR/prov-o/#Organization -->

    <owl:Class rdf:about="https://www.w3.org/TR/prov-o/#Organization">
        <rdfs:subClassOf rdf:resource="http://www.semanticweb.org/djlee/ontologies/2023/8/untitled-ontology-71#Group"/>
        <rdfs:comment>Used the Agent type - Organization</rdfs:comment>
    </owl:Class>
    


    <!-- https://www.w3.org/TR/prov-o/#Person -->

    <owl:Class rdf:about="https://www.w3.org/TR/prov-o/#Person">
        <rdfs:subClassOf rdf:resource="https://www.w3.org/TR/prov-o/#Agent"/>
        <rdfs:comment>Used to describe the Agent type Person.</rdfs:comment>
    </owl:Class>
    


    <!-- 
    ///////////////////////////////////////////////////////////////////////////////////////
    //
    // Individuals
    //
    ///////////////////////////////////////////////////////////////////////////////////////
     -->

    


    <!-- http://local.tamu.edu/djlee/ns/dqa#Accessability -->

    <owl:NamedIndividual rdf:about="http://local.tamu.edu/djlee/ns/dqa#Accessability">
        <rdf:type rdf:resource="http://local.tamu.edu/djlee/ns/dqa#ProductDimension"/>
        <rdfs:comment>The extent to which a data product can be accessed within a specific context of use, especially by individuals who require assistive technology or customized settings due to disabilities; The ability to perform as and when required.</rdfs:comment>
    </owl:NamedIndividual>
    


    <!-- http://local.tamu.edu/djlee/ns/dqa#Accuracy -->

    <owl:NamedIndividual rdf:about="http://local.tamu.edu/djlee/ns/dqa#Accuracy">
        <rdf:type rdf:resource="http://local.tamu.edu/djlee/ns/dqa#IntrinsicDimension"/>
        <rdfs:comment>The degree to which data is a correct or valid representation of an object, phenomenon, relation, process, or event.

Accuracy Scenario: Inaccurate data
Scenario: 
Alex a research scientist recently deposited his data. The data curation team at RDR Y after analyzing it found that the dataset&apos;s description in its ReadMe file doesn’t match what was submitted. This might be because the submitted version of the dataset was stale and not updated with any of the last-minute changes that Alex made in the data. 

Solution Scenario 1: Alex could use a version control tool to perform a last-minute check to verify if the most recent data was submitted to the RDR.  

Pros: Reduces human errors and also helps reduce confusion by automating a key manual task.
Cons: This could lead to confusion if there were too many versions with similar names

===================
Inaccurate version of the script used run the data leads to an accuracy problem in the associated data product. 

Scenario: Prof. Bret’s research team was using a script to run on their data. They were using a version control system like GitHub, and they had two threads in their Master repository; one was named “Main”, while the other was “Final”. Someone from the research team submitted the Final thread code of the script along with the data. When curators at RDR Y tried to run the code it did not work as expected. So they asked the team to look into it and initially, even they didn’t understand what was going on, but later figured out that they gave the wrong code as few people in the team thought “Main” was the actual code, while few thought “Final” was the actual code, mixing everything up.

Solution Scenario 2: Version control systems are made to make collaboration easier, however, improper naming conventions like “Main” and “Final” or “Actual Main” could easily confuse people. Prof. Bret after learning of this issue removed the redundant threads and made sure that proper naming conventions were followed from then on. He explained to the team what standard naming conventions they were to follow and made sure everyone understood them well.
Pros: By following good naming conventions, people can prevent many confusions and misunderstandings. 
Cons: This increases the need to think of good names for each thread, using standard conventions followed across the industry could help save some time.</rdfs:comment>
    </owl:NamedIndividual>
    


    <!-- http://local.tamu.edu/djlee/ns/dqa#Actionability -->

    <owl:NamedIndividual rdf:about="http://local.tamu.edu/djlee/ns/dqa#Actionability">
        <rdf:type rdf:resource="http://local.tamu.edu/djlee/ns/dqa#ProductDimension"/>
        <rdfs:comment>The ability of the identifier system to locate a data product using a unique and actionable identifier.</rdfs:comment>
    </owl:NamedIndividual>
    


    <!-- http://local.tamu.edu/djlee/ns/dqa#Completeness -->

    <owl:NamedIndividual rdf:about="http://local.tamu.edu/djlee/ns/dqa#Completeness">
        <rdf:type rdf:resource="http://local.tamu.edu/djlee/ns/dqa#IntrinsicDimension"/>
        <rdfs:comment>The extent to which data is a complete representation of another object, relation, process, or event.

========================
Metadata is incomplete. 
Scenario: Sam, a data curator working for RDR Y, once received a dataset that came along with metadata and a code. However, metadata is very sparse and incomplete, making it very difficult for him to understand the data and the code and the relationship between the two. So, he asked the research team to revise and expand the metadata, including the readme files for the data and the code.</rdfs:comment>
    </owl:NamedIndividual>
    


    <!-- http://local.tamu.edu/djlee/ns/dqa#Consistency -->

    <owl:NamedIndividual rdf:about="http://local.tamu.edu/djlee/ns/dqa#Consistency">
        <rdf:type rdf:resource="http://local.tamu.edu/djlee/ns/dqa#IntrinsicDimension"/>
        <rdfs:comment>The extent of consistency in using the same values or structure for representing an object, relation, process, or event.

=======
Consistency Scenario: Inconsistent names used for the same fields
Scenario 17: Henry a data curator at RDR Y, once had a dataset deposited that comprised multiple data files. Although the files were related, they used different naming conventions for their variables. In some files, gender data was under the header Gender, while in some places, it was under Sex. Similarly, with names, in some places, it was First name and Last name, while in some, it was First name and Surname. Henry talked to the research team and told them about the inconsistent naming conventions used across their datasets.</rdfs:comment>
    </owl:NamedIndividual>
    


    <!-- http://local.tamu.edu/djlee/ns/dqa#Credibility -->

    <owl:NamedIndividual rdf:about="http://local.tamu.edu/djlee/ns/dqa#Credibility">
        <rdf:type rdf:resource="http://local.tamu.edu/djlee/ns/dqa#ProductDimension"/>
        <rdfs:comment>The degree of reputation or credibility of a data product.</rdfs:comment>
    </owl:NamedIndividual>
    


    <!-- http://local.tamu.edu/djlee/ns/dqa#Currency -->

    <owl:NamedIndividual rdf:about="http://local.tamu.edu/djlee/ns/dqa#Currency">
        <rdf:type rdf:resource="http://local.tamu.edu/djlee/ns/dqa#IntrinsicDimension"/>
        <rdfs:comment>The age of data;
The extent to which the age of data meets the requirements of its usage context.</rdfs:comment>
    </owl:NamedIndividual>
    


    <!-- http://local.tamu.edu/djlee/ns/dqa#EthicalCompliance -->

    <owl:NamedIndividual rdf:about="http://local.tamu.edu/djlee/ns/dqa#EthicalCompliance">
        <rdf:type rdf:resource="http://local.tamu.edu/djlee/ns/dqa#ProductDimension"/>
        <rdfs:comment>The extent to which a data product complies with the ethical principles of a particular community or culture; 
The extent to which a data product preserves people’s privacy and does not disclose confidential information.


==========
Privacy scenario: Confidential/sensitive informaton included  in research data

Scenario: Oscar, a curator at RDR Y, got a dataset from Dr. Alex, a sociology researcher, that was populated using data derived from many social media platforms. This dataset contained some sensitive data like the neighborhoods where the users stay, and a few other details that could be direct identifiers. This is a privacy issue, so he had to sit with the research team and make sure that data was anonymized accordingly.</rdfs:comment>
    </owl:NamedIndividual>
    


    <!-- http://local.tamu.edu/djlee/ns/dqa#Integrity -->

    <owl:NamedIndividual rdf:about="http://local.tamu.edu/djlee/ns/dqa#Integrity">
        <rdf:type rdf:resource="http://local.tamu.edu/djlee/ns/dqa#ProductDimension"/>
        <rdfs:comment>The degree to which the integrity of a data product is preserved.</rdfs:comment>
    </owl:NamedIndividual>
    


    <!-- http://local.tamu.edu/djlee/ns/dqa#Interoperability -->

    <owl:NamedIndividual rdf:about="http://local.tamu.edu/djlee/ns/dqa#Interoperability">
        <rdf:type rdf:resource="http://local.tamu.edu/djlee/ns/dqa#ProductDimension"/>
        <rdfs:comment>The extent of a data product being interoperable and usable in another system;
The degree to which a data product has attributes that enable it to be installed, replaced, or moved from one system to another, preserving the existing quality in a specific context of use.</rdfs:comment>
    </owl:NamedIndividual>
    


    <!-- http://local.tamu.edu/djlee/ns/dqa#LegalCompliance -->

    <owl:NamedIndividual rdf:about="http://local.tamu.edu/djlee/ns/dqa#LegalCompliance">
        <rdf:type rdf:resource="http://local.tamu.edu/djlee/ns/dqa#ProductDimension"/>
        <rdfs:comment>The extent to which a data product complies with the rules, laws, and regulations of a particular community or a particular country.</rdfs:comment>
    </owl:NamedIndividual>
    


    <!-- http://local.tamu.edu/djlee/ns/dqa#Precision -->

    <owl:NamedIndividual rdf:about="http://local.tamu.edu/djlee/ns/dqa#Precision">
        <rdf:type rdf:resource="http://local.tamu.edu/djlee/ns/dqa#IntrinsicDimension"/>
        <rdfs:comment>The extent of precision/data of data in representing an object, relation, process, or event.</rdfs:comment>
    </owl:NamedIndividual>
    


    <!-- http://local.tamu.edu/djlee/ns/dqa#Recoverability -->

    <owl:NamedIndividual rdf:about="http://local.tamu.edu/djlee/ns/dqa#Recoverability">
        <rdf:type rdf:resource="http://local.tamu.edu/djlee/ns/dqa#ProductDimension"/>
        <rdfs:comment>The degree to which a data product has attributes that enable it to maintain and preserve a specified level of operations and quality, even in the event of failure, in a specific context of use.</rdfs:comment>
    </owl:NamedIndividual>
    


    <!-- http://local.tamu.edu/djlee/ns/dqa#Security -->

    <owl:NamedIndividual rdf:about="http://local.tamu.edu/djlee/ns/dqa#Security">
        <rdf:type rdf:resource="http://local.tamu.edu/djlee/ns/dqa#ProductDimension"/>
        <rdfs:comment>The degree to which a data product is appropriately protected from damage or abuse (including unauthorized use or access).</rdfs:comment>
    </owl:NamedIndividual>
    


    <!-- http://local.tamu.edu/djlee/ns/dqa#Simplicity -->

    <owl:NamedIndividual rdf:about="http://local.tamu.edu/djlee/ns/dqa#Simplicity">
        <rdf:type rdf:resource="http://local.tamu.edu/djlee/ns/dqa#IntrinsicDimension"/>
        <rdfs:comment>The extent of cognitive or representational complexity of data.</rdfs:comment>
    </owl:NamedIndividual>
    


    <!-- http://local.tamu.edu/djlee/ns/dqa#Traceability -->

    <owl:NamedIndividual rdf:about="http://local.tamu.edu/djlee/ns/dqa#Traceability">
        <rdf:type rdf:resource="http://local.tamu.edu/djlee/ns/dqa#ProductDimension"/>
        <rdfs:comment>The ability to trace the history, application, or location of a data product.</rdfs:comment>
    </owl:NamedIndividual>
    


    <!-- http://local.tamu.edu/djlee/ns/dqa#Understanability -->

    <owl:NamedIndividual rdf:about="http://local.tamu.edu/djlee/ns/dqa#Understanability">
        <rdf:type rdf:resource="http://local.tamu.edu/djlee/ns/dqa#ProductDimension"/>
        <rdfs:comment>The degree to which a data product has attributes that enable it to be read and interpreted by users.

Scenario
Oscar a junior data curator at RDR Y, recently received a dataset from Dr. Bert, this was highly complex data that had too many technical words, so Oscar had to frequently refer to the documentation and the metadata to understand the data. However, he noticed that some of the words mentioned in the documentation were equally difficult to understand since Oscar didn’t have any technical background in that particular field. Confused he asked his senior curators to help them out, but from a few particular words, codes, and formulas he had to contact Dr. Bert for guidance.

Solution scenari:
 It is important that researchers realize that technical jargon can be difficult for a lot of people to understand. Hence, when trying to write documentation about technical data it is important to use layman’s terms and give high-level explanations so that everyone is able to understand them.
Pros: This can dramatically increase the ease with which other people understand research data, while also reducing the need for rework.
Cons: By over-simplifying the documentation, the researcher might leave out a lot of crucial information that might reduce the important factor of the data among professionals in that field.

Solution scenario for the con
In such a case it is fruitful to develop two kinds of documentation, one explained in layman’s terms while the other explained using the technical words, in full depth and complexity appreciated by professionals of the field.</rdfs:comment>
    </owl:NamedIndividual>
</rdf:RDF>



<!-- Generated by the OWL API (version 4.5.9.2019-02-01T07:24:44Z) https://github.com/owlcs/owlapi -->

